trying to get ynotserve into everything.

examples/Data/LinkedListSeg.v
@@ -1,34 +1,30 @@
 Require Import Ynot.
 Require Import List.
+Require Import Peano_dec.
 
 Set Implicit Arguments.
 
 Open Local Scope hprop_scope.
 Open Local Scope stsepi_scope.
 
-Module Type DECIDABLE_DOMAIN.
-  Variables A : Set.
-  Variable  eq_a : forall (k1 k2: A), {k1 = k2} + {k1 <> k2}.
-End DECIDABLE_DOMAIN.
-
-Module LinkedListSegModel(A : DECIDABLE_DOMAIN).
- Export A.
+Section LinkedListSegModel.
+ Variable A : Set.
  Require Export List.
  Set Implicit Arguments.
 
- Definition head (ls : list A.A) :=
+ Definition head (ls : list A) :=
    match ls with
      | nil => None
      | x :: _ => Some x
    end.
  
- Definition tail (ls : list A.A) :=
+ Definition tail (ls : list A) :=
    match ls with
      | nil => nil
      | _ :: ls' => ls'
    end.
  
- Fixpoint insertAt_model (ls : list A.A) (a : A.A) (idx : nat) {struct idx} : list A.A :=
+ Fixpoint insertAt_model (ls : list A) (a : A) (idx : nat) {struct idx} : list A :=
    match idx with
      | 0 => a :: ls
      | S idx' => match ls with
@@ -37,26 +33,45 @@ Module LinkedListSegModel(A : DECIDABLE_DOMAIN).
                  end
   end.
 
-  Fixpoint removeFirst_model (ls : list A.A) (a : A.A) : list A.A :=
+Inductive action : Type :=
+  | Keep : action
+  | Del : action
+  | Update : A -> action.
+
+  Fixpoint process_model (ls : list A) (p : A -> action) : list A :=
+    match ls with
+      | nil => nil
+      | f :: r => 
+        match p f with
+          | Keep => f :: (process_model r p)
+          | Del => process_model r p
+          | Update f' => f' :: (process_model r p)
+        end
+    end.
+
+  Fixpoint foldr_model (T : Type) (p : A -> T -> T) (ls : list A) (t : T) {struct ls} : T :=
+    match ls with
+      | nil => t
+      | f :: r => p f (foldr_model p r t)
+    end.
+
+ Variable eq_a : forall (a b : A), {a = b} + {a <> b}.
+
+  Fixpoint removeFirst_model (ls : list A) (a : A) : list A :=
     match ls with
       | nil => nil
       | f :: r => if eq_a f a then r else f :: (removeFirst_model r a)
     end.
 
-  Fixpoint filter_model (ls : list A.A) (a : A.A) : list A.A :=
+  Fixpoint filter_model (ls : list A) (a : A) : list A :=
     match ls with 
       | nil => nil
       | f :: r => if eq_a f a then filter_model r a else f :: filter_model r a
     end.
-
 End LinkedListSegModel.
 
 Definition ptr_eq' : forall (p q : option ptr), {p = q} + {p <> q}.
   decide equality. apply ptr_eq_dec.
-Qed.
-
-Definition nat_eq : forall (p q : nat), {p = q} + {p <> q}.
-  decide equality.
 Qed.
 
 Definition maybe_points_to (p : option ptr) : hprop :=
@@ -67,92 +82,91 @@ Definition maybe_points_to (p : option ptr) : hprop :=
 
 Notation "x ~~>?" := (maybe_points_to x) (at level 38).
 
-Module Type LinkedListSeg.
-  Require Export List.
-  Declare Module A  : DECIDABLE_DOMAIN.
-  Module AL := LinkedListSegModel(A).
-  Import AL.
-
-  Require Export Ynot.
-  Open Scope hprop_scope.
-
-  Parameter llseg : option ptr -> option ptr -> list A.A -> hprop.
-  Definition llist (p: option ptr) (m : list A.A) := llseg p None m.
-
-  Parameter empty : STsep __ (fun r:option ptr => llseg r None nil).
-
-  Parameter cons : forall (v : A.A) (r : option ptr) (q : [option ptr])
-    (m : [list A.A]),
+Record LinkedListSeg (A : Set) := mkList
+  { LinkedList : Set := option ptr
+  ; llseg : LinkedList -> LinkedList -> list A -> hprop
+  ; llist := fun (p: LinkedList) (m : list A) => llseg p None m
+  ; empty : STsep __ (fun r:LinkedList => llseg r None nil)
+  ; cons : forall (v : A) (r : LinkedList) (q : [LinkedList]) (m : [list A]),
     STsep (q ~~ m ~~ llseg r q m * q ~~>?)
-          (fun r:option ptr => q ~~ m ~~ llseg r q (v :: m) * q ~~>?).
-
-  Parameter single : forall (v : A.A),
-    STsep __ (fun r:option ptr => llseg r None (v :: nil)).
-
-  Parameter freeList : forall (p' q : option ptr) (ls' : [list A.A]),
+          (fun r:LinkedList => q ~~ m ~~ llseg r q (v :: m) * q ~~>?)
+  ; single : forall (v : A),
+    STsep __ (fun r:LinkedList => llseg r None (v :: nil))
+  ; freeList : forall (p' q : LinkedList) (ls' : [list A]),
     STsep (ls' ~~ llseg p' q ls')
-          (fun _:unit => __).
-
-  Parameter freeHead : forall (p : option ptr) (q : [option ptr]) (b : [A.A])
-    (ls : [list A.A]),
+          (fun _:unit => __)
+  ; freeHead : forall (p : LinkedList) (q : [LinkedList]) (b : [A]) (ls : [list A]),
     STsep (ls ~~ q ~~ b ~~ llseg p q (b :: ls))
-          (fun r => ls ~~ q ~~ llseg r q ls).
-
-  Parameter append : forall (p q : option ptr) (lsp lsq : [list A.A]), 
+          (fun r => ls ~~ q ~~ llseg r q ls)
+  ; append : forall (p q : LinkedList) (lsp lsq : [list A]),
     STsep (lsp ~~ lsq ~~ llist p lsp * llist q lsq)
-          (fun r:option ptr => lsp ~~ lsq ~~ llist r (lsp ++ lsq)).
-
-  Parameter copy : forall (p q : option ptr) (ls : [list A.A]),
+          (fun r:LinkedList => lsp ~~ lsq ~~ llist r (lsp ++ lsq))
+  ; copy : forall (p q : LinkedList) (ls : [list A]),
     STsep (ls ~~ llseg p q ls * q ~~>?)
-          (fun r:option ptr => ls ~~ llseg p q ls * llseg r q ls * q ~~>?).
-
-  Parameter insertAt : forall (p : option ptr) (a : A.A) 
-    (idx : nat) (ls : [list A.A]),
+          (fun r:LinkedList => ls ~~ llseg p q ls * llseg r q ls * q ~~>?)
+  ; insertAt : forall (p : LinkedList) (a : A) (idx : nat) (ls : [list A]),
     STsep (ls ~~ llist p ls)
-          (fun r:option ptr => ls ~~ llist r (insertAt_model ls a idx)).
-
-  Parameter removeFirst : forall (p : option ptr) (a : A.A) (ls : [list A.A]),
-    STsep (ls ~~ llist p ls)
-          (fun r:option ptr => ls ~~ llist r (removeFirst_model ls a)).
-  
-  Parameter filter : forall (p : option ptr) (a : A.A) (ls : [list A.A]),
-    STsep (ls ~~ llist p ls)
-          (fun r:option ptr => ls ~~ llist r (filter_model ls a)).
-
-  Parameter elements : forall (p q : option ptr) (ls : [list A.A]),
+          (fun r:LinkedList => ls ~~ llist r (insertAt_model ls a idx))
+  ; elements : forall (p q : LinkedList) (ls : [list A]),
     STsep (ls ~~ llseg p q ls)
-          (fun r:list A.A => ls ~~ [r = ls] * llseg p q ls).
+          (fun r:list A => ls ~~ [r = ls] * llseg p q ls)
+  ; nil_empty : forall p q, llseg p q nil ==> [p = q]
+  ; removeFirst : forall (eq_a : forall (a b : A), {a = b} + {a <> b})
+    (p : LinkedList) (a : A) (ls : [list A]),
+    STsep (ls ~~ llist p ls)
+          (fun r:LinkedList => ls ~~ llist r (removeFirst_model eq_a ls a))
+  ; filter : forall (eq_a : forall (a b : A), {a = b} + {a <> b})
+    (p : LinkedList) (a : A) (ls : [list A]),
+    STsep (ls ~~ llist p ls)
+          (fun r:LinkedList => ls ~~ llist r (filter_model eq_a ls a))
+  ; process : forall (p q : LinkedList) (up : A -> action A) (ls : [list A]),
+    STsep (ls ~~ llseg p q ls)
+          (fun r:LinkedList => ls ~~ llseg r q (process_model ls up))
+  ; foldr_f : forall (T : Type) (p q : LinkedList) (f : A -> T -> T) (ls : [list A]) (t : T),
+    STsep (ls ~~ llseg p q ls)
+          (fun r:T => ls ~~ llseg p q ls * [r = foldr_model f ls t])
+  ; foldl : forall (T  : Type) (p q : LinkedList) (I : T -> list A -> hprop)
+    (c : forall (a : T) (v : A) (m : [list A]),
+         STsep (m ~~ I a m)
+               (fun a':T => m ~~ I a' (m ++ (v :: nil))))
+    (ls : [list A]) (a : T),
+    STsep (ls ~~ llseg p q ls * I a nil)
+          (fun r:T => ls ~~ llseg p q ls * I r ls)
+  ; foldr : forall (T  : Type) (p q : LinkedList) (I : T -> list A -> hprop)
+    (c : forall (a : T) (v : A) (m : [list A]),
+         STsep (m ~~ I a m)
+               (fun a':T => m ~~ I a' (v :: m)))
+    (ls : [list A]) (a : T),
+    STsep (ls ~~ llseg p q ls * I a nil)
+          (fun r:T => ls ~~ llseg p q ls * I r ls)
+  }.
 
-  Parameter nil_empty : forall p q, llseg p q nil ==> [p = q].
-End LinkedListSeg.
+Section HeapLinkedList.
+  Variable A : Set.
 
-Module HeapLinkedList(AD : DECIDABLE_DOMAIN) : LinkedListSeg with Module A := AD.
-  Module A := AD.
-  Module AL := LinkedListSegModel(A).
   Require Import Ynot.
-  Import AL.
 
   (** Representation ********************************************************)
 
-  Definition t : Set := AD.A.
-  Definition LinkedList : Set := option ptr.
+  Definition t : Set := A.
+  Definition LinkedList' : Set := option ptr.
 
   Record Node : Set := node {
     data: t;
-    next: LinkedList
+    next: LinkedList'
   }.
   
-  Fixpoint llseg (s e : LinkedList) (m : list t) {struct m} : hprop :=
+  Fixpoint llseg' (s e : LinkedList') (m : list t) {struct m} : hprop :=
     match m with 
       | nil => [s = e]
       | v :: r => [s <> e] *
         match s with
           | None => [False]
-          | Some p => Exists p' :@ LinkedList, p --> node v p' * llseg p' e r
+          | Some p => Exists p' :@ LinkedList', p --> node v p' * llseg' p' e r
         end
     end.
   
-  Definition llist (s : LinkedList) (m : list t) : hprop := llseg s None m.
+  Definition llist' (s : LinkedList') (m : list t) : hprop := llseg' s None m.
 
   (** Lemmas & Tactics ******************************************************)
 
@@ -160,60 +174,62 @@ Module HeapLinkedList(AD : DECIDABLE_DOMAIN) : LinkedListSeg with Module A := AD
     destruct nde; reflexivity.
   Qed.
   
-  Lemma head_tail : forall l f r,
+  Lemma head_tail : forall l (f:A) r,
     head l = Some f -> r = tail l -> l = f :: r.
     destruct l; intros;[ discriminate | simpl in *; congruence ] .
   Qed.
 
-  Lemma head_some_nonil : forall x y,
+  Lemma head_some_nonil : forall x (y:A),
     head x = Some y
     -> x <> nil.
     destruct x; intros; simpl in *; congruence.
+  Qed.
+
+  Lemma app_nil : forall T (x: list T), x ++ nil = x.
+    induction x; firstorder.
   Qed.
   
   Hint Resolve eta_node head_tail head_some_nonil.
 
   (**  Unfolding **)
-  Lemma llseg_unfold_nil : forall hd tl,
-    llseg hd tl nil ==> [hd = tl].
+  Lemma llseg'_unfold_nil : forall hd tl,
+    llseg' hd tl nil ==> [hd = tl].
     sep fail simpl.
   Qed.
 
-  Definition nil_empty := llseg_unfold_nil.
-
-  Lemma llseg_unfold_cons : forall hd tl ls v,
-    llseg hd tl (v :: ls) ==> Exists p :@ ptr, [hd = Some p] * Exists nde :@ Node,
-    p --> nde * [nde = node v (next nde)] * llseg (next nde) tl ls.
+  Lemma llseg'_unfold_cons : forall hd tl ls v,
+    llseg' hd tl (v :: ls) ==> Exists p :@ ptr, [hd = Some p] * Exists nde :@ Node,
+    p --> nde * [nde = node v (next nde)] * llseg' (next nde) tl ls.
     destruct ls; destruct hd; destruct tl; sep fail simpl. 
   Qed.
 
-  Lemma llseg_unfold_some_cons : forall p tl ls v,
-    llseg (Some p) tl (v :: ls) ==> Exists nde :@ Node,
-    p --> nde * [nde = node v (next nde)] * llseg (next nde) tl ls.
+  Lemma llseg'_unfold_some_cons : forall p tl ls v,
+    llseg' (Some p) tl (v :: ls) ==> Exists nde :@ Node,
+    p --> nde * [nde = node v (next nde)] * llseg' (next nde) tl ls.
     destruct ls; destruct tl; sep fail simpl. 
   Qed.
   
-  Lemma llseg_unfold_some : forall p tl ls,
+  Lemma llseg'_unfold_some : forall p tl ls,
     (Some p <> tl)
-    -> llseg (Some p) tl ls ==> Exists nde :@ Node,
-       p --> nde * [head ls = Some (data nde)] * llseg (next nde) tl (tail ls).
+    -> llseg' (Some p) tl ls ==> Exists nde :@ Node,
+       p --> nde * [head ls = Some (data nde)] * llseg' (next nde) tl (tail ls).
     destruct ls; sep fail simpl. 
   Qed.
 
-  Lemma llseg_unfold_same : forall p ls,
-    llseg p p ls ==> [ls = nil].
+  Lemma llseg'_unfold_same : forall p ls,
+    llseg' p p ls ==> [ls = nil].
     destruct ls; sep fail simpl.
   Qed.
 
-  Lemma llseg_unfold_head_none : forall p l,
-    llseg None p l ==> [p = None] * [l = nil].
+  Lemma llseg'_unfold_head_none : forall p l,
+    llseg' None p l ==> [p = None] * [l = nil].
     destruct l; sep fail simpl.
   Qed.
 
-  Lemma llseg_unfold_tail_none : forall p l,
+  Lemma llseg'_unfold_tail_none : forall p l,
     p <> None
-    -> llseg p None l ==> [l <> nil] * Exists p' :@ ptr, [p = Some p'] * 
-    Exists nde :@ Node, p' --> nde * llseg (next nde) None (tail l) * [head l = Some (data nde)].
+    -> llseg' p None l ==> [l <> nil] * Exists p' :@ ptr, [p = Some p'] * 
+    Exists nde :@ Node, p' --> nde * llseg' (next nde) None (tail l) * [head l = Some (data nde)].
     destruct l; destruct p; sep fail ltac:(try congruence).
   Qed.
   
@@ -221,16 +237,16 @@ Module HeapLinkedList(AD : DECIDABLE_DOMAIN) : LinkedListSeg with Module A := AD
   Lemma combine : forall nde ls p tl,
     Some p <> tl
     -> head ls = Some (data nde) 
-    -> p --> nde * llseg (next nde) tl (tail ls) ==> llseg (Some p) tl ls.
-    unfold llseg; destruct ls; intros; 
+    -> p --> nde * llseg' (next nde) tl (tail ls) ==> llseg' (Some p) tl ls.
+    unfold llseg'; destruct ls; intros; 
       [ inversion H0
         | sep fail auto; destruct nde; inversion H0; reflexivity ].
   Qed.
   
   Lemma combine' : forall nde ls p a n,
     a = data nde -> n = next nde
-    -> llseg n None ls * p --> nde ==> llseg (Some p) None (a :: ls).
-    unfold llseg; intros; assert (Some p <> None); try congruence; sep fail idtac.
+    -> llseg' n None ls * p --> nde ==> llseg' (Some p) None (a :: ls).
+    unfold llseg'; intros; assert (Some p <> None); try congruence; sep fail idtac.
   Qed.
 
   Hint Resolve combine combine'.
@@ -249,19 +265,19 @@ Module HeapLinkedList(AD : DECIDABLE_DOMAIN) : LinkedListSeg with Module A := AD
   Qed.
   
   Lemma neqseg : forall p ls q ls',
-    llseg (Some p) None ls * llseg q None ls' ==> [Some p <> q] * ??.
+    llseg' (Some p) None ls * llseg' q None ls' ==> [Some p <> q] * ??.
     destruct q; [ | sep fail ltac:(auto; try congruence) ].
     destruct ls; [ sep fail ltac:(auto; try congruence) | ].
     destruct ls'; [ sep fail ltac:(auto; try congruence) | ].
     simpl; inhabiter.
-    apply (@himp_trans ((llseg v0 None ls' * llseg v None ls) * (p0 --> node t1 v0 * p --> node t0 v))); [ sep fail auto | ].
+    apply (@himp_trans ((llseg' v0 None ls' * llseg' v None ls) * (p0 --> node t1 v0 * p --> node t0 v))); [ sep fail auto | ].
     apply (@himp_trans ([Some p <> Some p0] * (?? * ??))); [ | apply himp_frame; apply himp_split_any ].
     apply himp_comm_conc. apply himp_assoc_conc1. apply himp_split. sep fail auto. apply himp_comm_conc.
     apply (@himp_trans (p0 --> node t1 v0 * p --> node t0 v * [p0 <> p])); [ apply himp_disjoint | sep fail ltac:(auto; try congruence) ].
   Qed.
 
   Lemma somenone_seg : forall p ls,
-    llseg (Some p) None ls ==> [ls <> nil] * ??.
+    llseg' (Some p) None ls ==> [ls <> nil] * ??.
     destruct ls; sep fail auto; [ congruence | assert (t0 :: ls <> nil); [ firstorder | sep fail auto ] ].
   Qed.
   
@@ -279,15 +295,15 @@ Module HeapLinkedList(AD : DECIDABLE_DOMAIN) : LinkedListSeg with Module A := AD
   
   Lemma add_neqseg : forall p ls q ls' P Q,
     (Some p <> q -> 
-      (llseg (Some p) None ls * llseg q None ls' * P ==> Q))
-    -> llseg (Some p) None ls * llseg q None ls' * P ==> Q.
+      (llseg' (Some p) None ls * llseg' q None ls' * P ==> Q))
+    -> llseg' (Some p) None ls * llseg' q None ls' * P ==> Q.
     intros; apply (add_fact (@neqseg _ _ _ _) H).
   Qed.
 
   Lemma add_somenoneseg : forall p ls P Q,
     (ls <> nil ->
-      (llseg (Some p) None ls * P ==> Q))
-    -> llseg (Some p) None ls * P ==> Q.
+      (llseg' (Some p) None ls * P ==> Q))
+    -> llseg' (Some p) None ls * P ==> Q.
     intros; apply (add_fact (@somenone_seg _ _) H).
   Qed.
 
@@ -326,26 +342,26 @@ Module HeapLinkedList(AD : DECIDABLE_DOMAIN) : LinkedListSeg with Module A := AD
       end).
   
   Ltac add_segne :=
-    search_prem ltac:(idtac;fold llseg;
+    search_prem ltac:(idtac;fold llseg';
       match goal with
-        | [|- llseg ?X None ?XL * ?P ==> _] => 
+        | [|- llseg' ?X None ?XL * ?P ==> _] => 
           match P with 
-            | context H [llseg ?Y None ?YL] => let z := context H [__] in 
+            | context H [llseg' ?Y None ?YL] => let z := context H [__] in 
               match goal with 
                 | [ H: X = Y -> False |- _ ] => fail 1
                 | [ H: X <> Y |- _ ] => fail 1
                 | [ H: Y = X -> False |- _ ] => fail 1
                 | [ H: Y <> X |- _ ] => fail 1
-                | _ => apply (@himp_trans (llseg X None XL * llseg Y None YL * z));
+                | _ => apply (@himp_trans (llseg' X None XL * llseg' Y None YL * z));
                   [ solve [ sep fail auto ] | apply add_neqseg; intros ]
               end
           end
       end).
 
   Ltac add_somenoneseg :=
-    search_prem ltac:(idtac;fold llseg;
+    search_prem ltac:(idtac;fold llseg';
       match goal with
-        | [|- llseg (Some ?X) None ?XL * ?P ==> _] => 
+        | [|- llseg' (Some ?X) None ?XL * ?P ==> _] => 
           match goal with 
             | [ H: XL = nil -> False |- _ ] => fail 1
             | [ H: XL <> nil |- _ ] => fail 1
@@ -409,10 +425,10 @@ Module HeapLinkedList(AD : DECIDABLE_DOMAIN) : LinkedListSeg with Module A := AD
                          | Some _ => _
                        end] => destruct X
              | context[ptr_eq' ?X ?Y] => destruct (ptr_eq' X Y)
-             | context[llseg ?X ?X ?Y] => destruct Y; [ discriminate | ]
+             | context[llseg' ?X ?X ?Y] => destruct Y; [ discriminate | ]
            end
            || match CONC with
-                | context [llseg _ _ (match ?LS with 
+                | context [llseg' _ _ (match ?LS with 
                                         | nil => _
                                         | _ :: _ => _
                                       end)] =>
@@ -421,7 +437,7 @@ Module HeapLinkedList(AD : DECIDABLE_DOMAIN) : LinkedListSeg with Module A := AD
                     | [ H : head LS = Some _ |- _ ] => 
                       destruct LS; [ pose (head_some_nonil H); discriminate | ]
                   end 
-                | context [llseg _ _ ?LS] =>
+                | context [llseg' _ _ ?LS] =>
                   match goal with 
                     | [ H : head LS = Some ?HD |- _ ] => 
                       let RW := fresh "list_eq" in
@@ -466,28 +482,28 @@ Module HeapLinkedList(AD : DECIDABLE_DOMAIN) : LinkedListSeg with Module A := AD
 
   Ltac simplr := repeat simplr''.
 
-  Ltac llseg_unfolding := 
+  Ltac llseg'_unfolding := 
     match goal with 
       [ |- ?T ==> _ ] =>
       match T with
-        | llseg _ _ nil => apply llseg_unfold_nil
-        | llseg (Some _) _ (_ :: _) => apply llseg_unfold_some_cons
-        | llseg (Some _) _ _ => apply llseg_unfold_some; try solve [congruence]
-        | llseg _ _ (_ :: _) => apply llseg_unfold_cons
-        | llseg ?p ?p _ => apply llseg_unfold_same
-        | llseg None _ _ => apply llseg_unfold_head_none
-        | llseg _ None _ => apply llseg_unfold_tail_none ; solve [congruence]
+        | llseg' _ _ nil => apply llseg'_unfold_nil
+        | llseg' (Some _) _ (_ :: _) => apply llseg'_unfold_some_cons
+        | llseg' (Some _) _ _ => apply llseg'_unfold_some; try solve [congruence]
+        | llseg' _ _ (_ :: _) => apply llseg'_unfold_cons
+        | llseg' ?p ?p _ => apply llseg'_unfold_same
+        | llseg' None _ _ => apply llseg'_unfold_head_none
+        | llseg' _ None _ => apply llseg'_unfold_tail_none ; solve [congruence]
       end
     end.
 
-  Ltac unfolder := simpl_prem ltac:(idtac; llseg_unfolding).
+  Ltac unfolder := simpl_prem ltac:(idtac; llseg'_unfolding).
 
   Ltac simp_prem := discriminate || (repeat (ondemand_subst || unfolder || expander)).
 
-  Ltac t := unfold llist; simpl_IfNull; sep simp_prem simplr; sep fail auto.
-  Ltac f := fold llseg; fold llist.
+  Ltac t := unfold llist'; simpl_IfNull; sep simp_prem simplr; sep fail auto.
+  Ltac f := fold llseg'; fold llist'.
 
-  Ltac rsep expander tac := unfold llist; intros;
+  Ltac rsep expander tac := unfold llist'; intros;
     try equater; try inhabiter; try unpack_conc; try canceler; try expander;
       repeat match goal with
                | [ H1 : ?X = [?Y]%inhabited, H2 : inhabit_unpack ?X ?XV = [?Z]%inhabited |- _ ==> ?CONC ] => 
@@ -500,33 +516,33 @@ Module HeapLinkedList(AD : DECIDABLE_DOMAIN) : LinkedListSeg with Module A := AD
       solve [ sep fail idtac | tac ].
   Debug Off.
   (** Implementation *********************************************************)
-  Definition empty : STsep __ (fun r:LinkedList => llseg r None nil).
+  Definition empty' : STsep __ (fun r:LinkedList' => llseg' r None nil).
     refine ({{Return None}});
       t.  
   Qed.
 
-  Definition cons : forall (v : A) (r : LinkedList) (q : [LinkedList])
+  Definition cons' : forall (v : A) (r : LinkedList') (q : [LinkedList'])
     (m : [list t]),
-    STsep (q ~~ m ~~ llseg r q m * q ~~>?)
-          (fun r:LinkedList => 
-              q ~~ m ~~ llseg r q (v :: m) * q ~~>?).
-    intros;
-    refine (l <- New (node v r); {{Return (Some l)}});
+    STsep (q ~~ m ~~ llseg' r q m * q ~~>?)
+          (fun r:LinkedList' => 
+              q ~~ m ~~ llseg' r q (v :: m) * q ~~>?).
+    refine (fun v r q m =>
+      l <- New (node v r);
+      {{ Return (Some l) }});
       t.
   Qed.
 
-  Definition single : forall (v : t),
-    STsep __ (fun r:LinkedList => llseg r None (v :: nil)).
-    refine (fun v => {{cons v None [None] [nil]}});
+  Definition single' : forall (v : t),
+    STsep __ (fun r:LinkedList' => llseg' r None (v :: nil)).
+    refine (fun v => {{ cons' v None [None] [nil] }});
       t.
   Qed.
 
-  Definition freeHead : forall (p : LinkedList) (q : [LinkedList]) (b : [t])
+  Definition freeHead' : forall (p : LinkedList') (q : [LinkedList']) (b : [t])
     (ls : [list t]),
-    STsep (ls ~~ q ~~ b ~~ llseg p q (b :: ls))
-          (fun r => ls ~~ q ~~ llseg r q ls).
-    intros;
-    refine (
+    STsep (ls ~~ q ~~ b ~~ llseg' p q (b :: ls))
+          (fun r => ls ~~ q ~~ llseg' r q ls).
+    refine (fun p q b ls =>
       IfNull p Then {{!!!}}
       Else nde <- !p;
            Free p;;
@@ -534,44 +550,43 @@ Module HeapLinkedList(AD : DECIDABLE_DOMAIN) : LinkedListSeg with Module A := AD
     t.
   Qed.
 
-  Definition freeList : forall (p' q : LinkedList) (ls' : [list t]),
-    STsep (ls' ~~ llseg p' q ls')
+  Definition freeList' : forall (p' q : LinkedList') (ls' : [list t]),
+    STsep (ls' ~~ llseg' p' q ls')
           (fun _:unit => __).
-    intros.
-    refine (Fix2
-      (fun p ls => ls ~~ llseg p q ls)
-      (fun p ls (_:unit) => __)
-      (fun self p ls =>
-        if ptr_eq' p q then 
-          {{Return tt}}
-        else
-          IfNull p Then
-            {{!!!}}
-          Else
-            nde <- !p;
-            Free p;;
-            self (next nde) (ls ~~~ tail ls)
-            )
-      p' ls');
+    refine (fun p' q ls' =>
+      Fix2 (fun p ls => ls ~~ llseg' p q ls)
+           (fun p ls (_:unit) => __)
+           (fun self p ls =>
+             if ptr_eq' p q then 
+               {{Return tt}}
+             else
+               IfNull p Then
+                 {{!!!}}
+               Else
+                 nde <- !p;
+                 Free p;;
+                 self (next nde) (ls ~~~ tail ls))
+           p' ls');
     clear self; t.
   Qed.
 
-  Definition elements : forall (p q : option ptr) (ls : [list A.A]),
-    STsep (ls ~~ llseg p q ls)
-          (fun r:list A.A => ls ~~ [r = ls] * llseg p q ls).
-    intros.
-    refine (Fix2 (fun p ls => ls ~~ llseg p q ls)
-                 (fun p ls (r : list A.A) => ls ~~ [r = ls] * llseg p q ls)
-                 (fun self p ls =>
-                   if ptr_eq' p q
-                   then {{Return nil}}
-                   else 
-                     IfNull p
-                     Then {{!!!}}
-                     Else nde <- !p;
-                          rr <- self (next nde) (ls ~~~ tail ls) <@> (ls ~~ p --> nde * [head ls = Some (data nde)]);
-                          {{Return (data nde :: rr)}})
-                 p ls);
+  Definition elements' : forall (p q : LinkedList') (ls : [list A]),
+    STsep (ls ~~ llseg' p q ls)
+          (fun r:list A => ls ~~ [r = ls] * llseg' p q ls).
+    refine (fun p q ls =>
+      Fix2 (fun p ls => ls ~~ llseg' p q ls)
+           (fun p ls (r : list A) => ls ~~ [r = ls] * llseg' p q ls)
+           (fun self p ls =>
+             if ptr_eq' p q then
+               {{Return nil}}
+             else 
+               IfNull p Then
+                 {{!!!}}
+               Else 
+                 nde <- !p;
+                 rr <- self (next nde) (ls ~~~ tail ls) <@> (ls ~~ p --> nde * [head ls = Some (data nde)]);
+                 {{Return (data nde :: rr)}})
+           p ls);
     try clear self; solve [ t ].
   Qed.
 
@@ -581,112 +596,288 @@ Module HeapLinkedList(AD : DECIDABLE_DOMAIN) : LinkedListSeg with Module A := AD
       try match goal with
             | [ |- _ ==> ?CONC ] => 
               match CONC with 
-                | context [llseg _ _ (?X ++ _)] => destruct X
+                | context [llseg' _ _ (?X ++ _)] => destruct X
               end
           end; sep fail simplr.
     
-    Definition append' : forall (pr' : ptr) (nde' : Node) (q : LinkedList)
+    Definition append_help' : forall (pr' : ptr) (nde' : Node) (q : LinkedList')
       (lsp' lsq : [list t]),
-      STsep (lsp' ~~ lsq ~~ pr' --> nde' * llist (next nde') lsp' * llist q lsq)
-            (fun _:unit => lsp' ~~ lsq ~~ Exists r :@ LinkedList, 
-                pr' --> node (data nde') r * llist r (lsp' ++ lsq)).
-      intros;
-      refine (Fix3
-        (fun pr nde lsp => 
-          lsp ~~ lsq ~~ pr --> nde * llist (next nde) lsp * llist q lsq)
-        (fun pr nde lsp (_:unit) => 
-          lsp ~~ lsq ~~ Exists r :@ LinkedList, pr --> node (data nde) r * 
-          llist r (lsp ++ lsq))
-        (fun self pr nde lsp =>
-          IfNull (next nde) As p
-          Then {{pr ::= node (data nde) q}}
-          Else nde' <- !p;
-               {{self p nde' (lsp ~~~ tail lsp) <@> _}}
-        ) pr' nde' lsp');
+      STsep (lsp' ~~ lsq ~~ pr' --> nde' * llist' (next nde') lsp' * llist' q lsq)
+            (fun _:unit => lsp' ~~ lsq ~~ Exists r :@ LinkedList', 
+                pr' --> node (data nde') r * llist' r (lsp' ++ lsq)).
+      refine (fun pr' nde' q lsp' lsq =>
+        Fix3 (fun pr nde lsp => 
+               lsp ~~ lsq ~~ pr --> nde * llist' (next nde) lsp * llist' q lsq)
+             (fun pr nde lsp (_:unit) => 
+               lsp ~~ lsq ~~ Exists r :@ LinkedList', pr --> node (data nde) r * 
+               llist' r (lsp ++ lsq))
+             (fun self pr nde lsp =>
+               IfNull (next nde) As p Then
+                 {{pr ::= node (data nde) q}}
+               Else 
+                 nde' <- !p;
+                 {{self p nde' (lsp ~~~ tail lsp) <@> _}})
+             pr' nde' lsp');
       solve [ rsep simp_prem q ].
     Qed.
 
-    Definition append : forall (p q : LinkedList) (lsp lsq : [list t]), 
-      STsep (lsp ~~ lsq ~~ llist p lsp * llist q lsq)
-            (fun r:LinkedList => lsp ~~ lsq ~~ llist r (lsp ++ lsq)).
-      intros;
-      refine (
-        IfNull p As p'
-        Then {{Return q}}
-        Else nde <- !p';
-             append' p' nde q (lsp ~~~ tail lsp) lsq <@> _;;
-             {{Return p}});
+    Definition append' : forall (p q : LinkedList') (lsp lsq : [list t]), 
+      STsep (lsp ~~ lsq ~~ llist' p lsp * llist' q lsq)
+            (fun r:LinkedList' => lsp ~~ lsq ~~ llist' r (lsp ++ lsq)).
+      refine (fun p q lsp lsq =>
+        IfNull p As p' Then
+          {{Return q}}
+        Else 
+          nde <- !p';
+          append_help' p' nde q (lsp ~~~ tail lsp) lsq <@> _;;
+          {{Return p}});
       rsep simp_prem q.
     Qed.
 
   End append.
 
-  Definition copy : forall (p' q : LinkedList) (ls' : [list t]),
-    STsep (ls' ~~ llseg p' q ls' * q ~~>?)
-          (fun r:LinkedList => ls' ~~ llseg p' q ls' * llseg r q ls' * q ~~>?).
-    intros;
-    refine (Fix2
-      (fun p ls   => ls ~~ llseg p q ls * q ~~>?)
-      (fun p ls r => ls ~~ llseg p q ls * llseg r q ls * q ~~>?)
-      (fun self p ls =>
-        if ptr_eq' p q then
-          {{Return q}}
-        else
-          IfNull p Then {{!!!}}
-          Else nde <- !p;
-               rr <- self (next nde) (ls ~~~ tail ls) <@> _;
-               res <- cons (data nde) rr [q] (ls ~~~ tail ls) <@> _;
-               {{Return res}}) p' ls');
+  Definition copy' : forall (p' q : LinkedList') (ls' : [list t]),
+    STsep (ls' ~~ llseg' p' q ls' * q ~~>?)
+          (fun r:LinkedList' => ls' ~~ llseg' p' q ls' * llseg' r q ls' * q ~~>?).
+    refine (fun p' q ls' =>
+      Fix2 (fun p ls   => ls ~~ llseg' p q ls * q ~~>?)
+           (fun p ls r => ls ~~ llseg' p q ls * llseg' r q ls * q ~~>?)
+           (fun self p ls =>
+             if ptr_eq' p q then
+               {{Return q}}
+             else
+               IfNull p Then
+                 {{!!!}}
+               Else 
+                 nde <- !p;
+                 rr <- self (next nde) (ls ~~~ tail ls) <@> _;
+                 res <- cons' (data nde) rr [q] (ls ~~~ tail ls) <@> _;
+                 {{Return res}}) p' ls');
     clear self; solve [ rsep simp_prem simplr | t ].
   Qed.
 
-  Definition insertAt' : forall (p' : ptr) (idx' : nat) (a : A) 
+  Definition insertAt_help' : forall (p' : ptr) (idx' : nat) (a : A) 
     (ls' : [list t]),
-    STsep (ls' ~~ llist (Some p') ls')
+    STsep (ls' ~~ llist' (Some p') ls')
           (fun _:unit => 
-              ls' ~~ llist (Some p') (insertAt_model ls' a (S idx'))).
-    intros;
-    refine (Fix3 
-      (fun p ls idx => ls ~~ llist (Some p) ls)
-      (fun p ls idx (_:unit) =>
-          ls ~~ llist (Some p) (insertAt_model ls a (S idx)))
-      (fun self p ls idx =>
-        nde <- !p;
-        if nat_eq 0 idx then
-          nelem <- New (node a (next nde));
-          p ::= node (data nde) (Some nelem);;
-          {{Return tt}}
-        else
-          IfNull next nde As nxt Then 
-            nelem <- New (node a (next nde));
-            p ::= node (data nde) (Some nelem);;
-            {{Return tt}}
-          Else
-            {{self nxt (ls ~~~ tail ls) (pred idx) <@> 
-              (ls ~~ p --> nde * [head ls = Some (data nde)])}})
-      p' ls' idx');
+              ls' ~~ llist' (Some p') (insertAt_model ls' a (S idx'))).
+    refine (fun p' idx' a ls' =>
+      Fix3 (fun p ls idx => ls ~~ llist' (Some p) ls)
+           (fun p ls idx (_:unit) =>
+             ls ~~ llist' (Some p) (insertAt_model ls a (S idx)))
+           (fun self p ls idx =>
+             nde <- !p;
+             if eq_nat_dec 0 idx then
+               nelem <- New (node a (next nde));
+               p ::= node (data nde) (Some nelem);;
+               {{Return tt}}
+             else
+               IfNull next nde As nxt Then 
+                 nelem <- New (node a (next nde));
+                 p ::= node (data nde) (Some nelem);;
+                 {{Return tt}}
+               Else
+                 {{self nxt (ls ~~~ tail ls) (pred idx) <@> 
+                     (ls ~~ p --> nde * [head ls = Some (data nde)])}})
+           p' ls' idx');
     clear self; solve [ t | t; destruct idx; t ].
   Qed.
 
-  Definition insertAt : forall (p : LinkedList) (a : t) (idx : nat)
+  Definition insertAt' : forall (p : LinkedList') (a : t) (idx : nat)
     (ls : [list t]),
-    STsep (ls ~~ llist p ls)
-          (fun r:LinkedList => ls ~~ llist r (insertAt_model ls a idx)).
-    intros; refine (
-      IfNull p
-      Then {{cons a p [None] ls <@> (ls ~~ [ls = nil])}}
-      Else if nat_eq idx 0 then
-             {{cons a (Some p) [None] ls <@> __}}
-           else
-             insertAt' p (pred idx) a ls <@> __;;
-             {{Return (Some p)}});
-  solve [ t | destruct idx; t ].
+    STsep (ls ~~ llist' p ls)
+          (fun r:LinkedList' => ls ~~ llist' r (insertAt_model ls a idx)).
+    refine (fun p a idx ls =>
+      IfNull p Then 
+        {{ cons' a p [None] ls <@> (ls ~~ [ls = nil]) }}
+      Else 
+        if eq_nat_dec idx 0 then
+          {{ cons' a (Some p) [None] ls <@> __ }}
+        else
+          insertAt_help' p (pred idx) a ls <@> __;;
+          {{ Return (Some p) }});
+    solve [ t | destruct idx; t ].
   Qed.
 
+  Section Process.
+
+    Ltac q := t;
+      match goal with 
+        | [ |- context[llseg' _ _ (process_model ?X _)] ] => 
+          match X with
+            | tail _ => fail 1
+            | _ => destruct X;
+              [ match goal with
+                  | [ H : head nil = Some _ |- _ ] => inversion H
+                end
+              | t; match goal with
+                     | [ H : _ = Keep _ |- _ ] => rewrite H
+                     | [ H : _ = Del _ |- _ ] => rewrite H
+                     | [ H : _ = Update _ |- _ ] => rewrite H
+                   end; t ]
+          end
+      end.
+
+    Definition process_help' : forall (prev' : ptr) (prev_a' : t) (up : t -> action t)
+      (p' q : LinkedList') (ls' : [list A]),
+      STsep (ls' ~~ llseg' p' q ls' * prev' --> node prev_a' p')
+            (fun (_:unit) => ls' ~~ Exists r :@ LinkedList', 
+                llseg' r q (process_model ls' up) * prev' --> node prev_a' r).
+      refine (fun prev' prev_a' up p' q ls' =>
+        Fix4 (fun prev prev_a p ls => ls ~~ llseg' p q ls * prev --> node prev_a p)
+             (fun prev prev_a p ls (_:unit) => ls ~~ Exists r :@ LinkedList', 
+               llseg' r q (process_model ls up) * prev --> node prev_a r)
+             (fun self prev prev_a p ls =>
+               if ptr_eq' p q then
+                 {{ Return tt }}
+               else
+                 IfNull p As p' Then
+                   {{ !!! }}
+                 Else
+                   nde <- !p';
+                   match up (data nde) as act 
+                     return STsep (ls ~~ llseg' (next nde) q (tail ls) * prev --> node prev_a (Some p') * 
+                                    p' --> node (data nde) (next nde) * [up (data nde) = act] * [head ls = Some (data nde)])
+                                  (fun (_:unit) => ls ~~ Exists r :@ LinkedList', 
+                                    llseg' r q (process_model ls up) * prev --> node prev_a r)
+                 with
+                 | Keep => 
+                   {{self p' (data nde) (next nde) (ls ~~~ tail ls) <@> 
+                     (ls ~~ [head ls = Some (data nde)] * [p = Some p'] * 
+                       prev --> node prev_a p * [up (data nde) = Keep t])}}
+                 | Del =>
+                   prev ::=  node prev_a (next nde);; 
+                   Free p';;
+                   {{self prev prev_a (next nde) (ls ~~~ tail ls) <@> 
+                     (ls ~~ [head ls = Some (data nde)] * [p = Some p'] * [up (data nde) = Del t])}}
+                 | Update val' =>
+                   p' ::= node val' (next nde);;
+                   {{self p' val' (next nde) (ls ~~~ tail ls) <@>
+                     (ls ~~ prev --> node prev_a p * [head ls = Some (data nde)] * [up (data nde) = Update val'])}}
+               end
+      ) prev' prev_a' p' ls');
+      solve [ q ].
+    Qed.
+
+    Definition process' : forall (p q : LinkedList') (up : A -> action t) (ls : [list A]),
+      STsep (ls ~~ llseg' p q ls)
+            (fun r:LinkedList' => ls ~~ llseg' r q (process_model ls up)).
+      refine (fun p q up ls =>
+        if ptr_eq' p q then
+          {{ Return p }}
+        else
+          IfNull p As p' Then
+            {{ !!! }}
+          Else
+            nde <- !p';
+            {{ process_help' p' (data nde) up (next nde) q (ls ~~~ tail ls) <@> 
+                 (ls ~~ [head ls = Some (data nde)]) }};;
+            match up (data nde) as act 
+              return STsep (ls ~~ Exists r :@ LinkedList', p' --> node (data nde) r * 
+                              llseg' r q (process_model (tail ls) up) * [head ls = Some (data nde)] * [up (data nde) = act])
+                           (fun (r:LinkedList') => ls ~~ llseg' r q (process_model ls up))
+              with
+              | Keep => {{ Return p }}
+              | Del =>
+                nde <- !p';
+                Free p';;
+                {{ Return (next nde) }}
+              | Update val' =>
+                nde <- !p';
+                p' ::= node val' (next nde);;
+                {{ Return (Some p') }}
+            end); 
+      solve [ q ].
+    Qed.
+  End Process.
+
+  Section Fold.
+
+    Definition foldr_f' : forall (T : Type) (p q : LinkedList') (f : A -> T -> T) (ls : [list A]) (t : T),
+      STsep (ls ~~ llseg' p q ls)
+            (fun r:T => ls ~~ llseg' p q ls * [r = foldr_model f ls t]).
+      refine (fun T p q f ls t =>
+        Fix2 (fun p ls => ls ~~ llseg' p q ls)
+             (fun p ls res => ls ~~ llseg' p q ls * [res = foldr_model f ls t])
+             (fun self p ls =>
+               if ptr_eq' p q then
+                 {{ Return t }}
+               else
+                 IfNull p As p' Then
+                   {{ !!! }}
+                 Else
+                   nde <- !p';
+                   r <- self (next nde) (ls ~~~ tail ls) <@> (ls ~~ p' --> nde * [head ls = Some (data nde)]) ;
+                   {{ Return (f (data nde) r) }})
+             p ls); try clear self;
+      solve [ t ].
+    Qed.
+
+    Definition foldl' : forall (T  : Type) (p q : LinkedList') (I : T -> list A -> hprop)
+      (c : forall (a : T) (v : A) (m : [list A]),
+           STsep (m ~~ I a m)
+                 (fun a':T => m ~~ I a' (m ++ (v :: nil))))
+      (ls' : [list A]) (a : T),
+      STsep (ls' ~~ llseg' p q ls' * I a nil)
+            (fun r:T => ls' ~~ llseg' p q ls' * I r ls').
+      refine (fun T p q I c ls' a =>
+        {{ Fix4 (fun acc beg p ls => ls' ~~ beg ~~ ls ~~ llseg' p q ls * I acc beg * [ls' = beg ++ ls])
+                (fun _   beg p ls res => ls' ~~ beg ~~ ls ~~ llseg' p q ls * I res ls' * [ls' = beg ++ ls])
+                (fun self acc beg p ls =>
+                  if ptr_eq' p q then
+                    {{ Return acc }}
+                  else
+                    IfNull p As p' Then
+                      {{ !!! }}
+                    Else
+                      nde <- !p' ;
+                      acc' <- @c acc (data nde) beg <@> (ls ~~ beg ~~ ls' ~~ [head ls = Some (data nde)] * llseg' (next nde) q (tail ls) * 
+                                                           [ls' = beg ++ ls] * p' --> nde) (** sep forgets information **);
+                      res <- self acc' (inhabit_unpack2 beg ls (fun beg ls => match ls with 
+                                                                                | nil => nil
+                                                                                | a :: b => beg ++ (a :: nil)
+                                                                              end)) (next nde) (ls ~~~ tail ls) <@> (ls ~~ [head ls = Some (data nde)] * _) ;
+                      {{Return res}} )
+                a (inhabits (@nil A)) p ls'}}); try clear self;
+      solve [ t 
+            | t; rewrite app_nil; t
+            | t; rewrite app_ass; t
+            | t; destruct x; simpl in *; [ discriminate | rewrite app_ass; simpl in *; t ]].
+    Qed.
+
+    Definition foldr' : forall (T  : Type) (p q : LinkedList') (I : T -> list A -> hprop)
+      (c : forall (a : T) (v : A) (m : [list A]),
+           STsep (m ~~ I a m)
+                 (fun a':T => m ~~ I a' (v :: m)))
+      (ls' : [list A]) (a : T),
+      STsep (ls' ~~ llseg' p q ls' * I a nil)
+            (fun r:T => ls' ~~ llseg' p q ls' * I r ls').
+      refine (fun T p q I c ls' a =>
+        {{ Fix2 (fun p ls => ls ~~ llseg' p q ls * I a nil)
+                (fun p ls res => ls ~~ llseg' p q ls * I res ls)
+                (fun self p ls =>
+                  if ptr_eq' p q then
+                    {{ Return a }}
+                  else
+                    IfNull p As p' Then
+                      {{ !!! }}
+                    Else
+                      nde <- !p' ;
+                      rr  <- self (next nde) (ls ~~~ tail ls) <@> ((ls ~~ [head ls = Some (data nde)]) * _) ;
+                      res <- @c rr (data nde) (ls ~~~ tail ls) <@> (ls ~~ llseg' p q ls * [head ls = Some (data nde)]);
+                      {{Return res}})
+                p ls'}}); try clear self;
+      solve [ t ].
+    Qed.
+
+  End Fold.
+
+
   Section Remove.
+    Variable eq_a : forall (a b : A), {a = b} + {a <> b}.
     Ltac q := t; 
       match goal with
-        | [ |- context[llseg _ _ (filter_model ?X _)] ] => 
+        | [ |- context[llseg' _ _ (filter_model _ ?X _)] ] => 
           match X with
             | tail _ => fail 1
             | _ => destruct X; simpl; 
@@ -694,7 +885,7 @@ Module HeapLinkedList(AD : DECIDABLE_DOMAIN) : LinkedListSeg with Module A := AD
                     | [ |- context[eq_a ?X ?Y] ] => destruct (eq_a X Y)
                   end; t
           end
-        | [ |- context[llseg _ _ (removeFirst_model ?X _)] ] => 
+        | [ |- context[llseg' _ _ (removeFirst_model _ ?X _)] ] => 
           match X with
             | tail _ => fail 1
             | _ => destruct X; simpl; 
@@ -704,98 +895,100 @@ Module HeapLinkedList(AD : DECIDABLE_DOMAIN) : LinkedListSeg with Module A := AD
           end
       end.
 
-    Definition removeFirst' : forall (pr' : ptr) (p' : LinkedList) 
+    Definition removeFirst_help' : forall (pr' : ptr) (p' : LinkedList') 
       (pr_a' a : t) (ls' : [list t]),
-      STsep (ls' ~~ llist p' ls' * pr' --> node pr_a' p')
-            (fun _:unit => ls' ~~ Exists p'' :@ LinkedList, 
-                llist p'' (removeFirst_model ls' a) * pr' --> node pr_a' p'').
-      intros;
-      refine (Fix4
-        (fun pr pr_a p ls => ls ~~ llist p ls * pr --> node pr_a p)
-        (fun pr pr_a p ls r => ls ~~ Exists p'' :@ LinkedList, 
-            llist p'' (removeFirst_model ls a) * pr --> node pr_a p'')
-        (fun self pr pr_a p ls =>
-          IfNull p As p'
-          Then {{Return tt}}
-          Else nde <- !p';
-               if eq_a (data nde) a then 
-                 pr ::=  node pr_a (next nde);;
-                 Free p';;
-                 {{Return tt}}
-               else 
-                 {{self p' (data nde) (next nde) (ls ~~~ tail ls) <@> 
-                   (ls ~~ [head ls = Some (data nde)] * [ls <> nil] * 
-                     [p = Some p'] * pr --> node pr_a p)}}
-        ) pr' pr_a' p' ls');
+      STsep (ls' ~~ llist' p' ls' * pr' --> node pr_a' p')
+            (fun _:unit => ls' ~~ Exists p'' :@ LinkedList', 
+                llist' p'' (removeFirst_model eq_a ls' a) * pr' --> node pr_a' p'').
+      refine (fun pr' p' pr_a' a ls' =>
+        Fix4 (fun pr pr_a p ls => ls ~~ llist' p ls * pr --> node pr_a p)
+             (fun pr pr_a p ls r => ls ~~ Exists p'' :@ LinkedList', 
+               llist' p'' (removeFirst_model eq_a ls a) * pr --> node pr_a p'')
+             (fun self pr pr_a p ls =>
+               IfNull p As p' Then
+                 {{ Return tt }}
+               Else nde <- !p';
+                 if eq_a (data nde) a then 
+                   pr ::=  node pr_a (next nde);;
+                   Free p';;
+                   {{ Return tt }}
+                 else 
+                   {{ self p' (data nde) (next nde) (ls ~~~ tail ls) <@> 
+                        (ls ~~ [head ls = Some (data nde)] * [ls <> nil] * 
+                          [p = Some p'] * pr --> node pr_a p) }}
+             ) pr' pr_a' p' ls');
       clear self; q.
     Qed.
 
-    Definition removeFirst : forall (p : LinkedList) (a : t) (ls : [list t]),
-      STsep (ls ~~ llist p ls)
-            (fun r:LinkedList => ls ~~ llist r (removeFirst_model ls a)).
-      intros;
-      refine (
-        IfNull p As p'
-        Then {{Return p}}
+    Definition removeFirst' : forall (p : LinkedList') (a : t) (ls : [list t]),
+      STsep (ls ~~ llist' p ls)
+            (fun r:LinkedList' => ls ~~ llist' r (removeFirst_model eq_a ls a)).
+      refine (fun p a ls =>
+        IfNull p As p' Then
+          {{ Return p }}
         Else nde <- !p';
-             if eq_a (data nde) a then 
-               Free p';;
-               {{Return (next nde)}}
-             else
-               removeFirst' p' (next nde) (data nde) a (ls ~~~ tail ls) <@>
-                 (ls ~~ [head ls = Some (data nde)]);;
-               {{Return p}});
+          if eq_a (data nde) a then 
+            Free p';;
+            {{ Return (next nde) }}
+          else
+            removeFirst_help' p' (next nde) (data nde) a (ls ~~~ tail ls) <@>
+               (ls ~~ [head ls = Some (data nde)]);;
+            {{ Return p }});
       q.
     Qed.
 
-
-    Definition filter' : forall (pr' : ptr) (p' : LinkedList) (pr_a' a : t)
+    Definition filter_help' : forall (pr' : ptr) (p' : LinkedList') (pr_a' a : t)
       (ls' : [list t]),
-      STsep (ls' ~~ llist p' ls' * pr' --> node pr_a' p')
-            (fun (_:unit) => ls' ~~ Exists r :@ LinkedList, 
-                llist r (filter_model ls' a) * pr' --> node pr_a' r).
-      intros;
-      refine (Fix4
-        (fun pr pr_a p ls => ls ~~ llist p ls * pr --> node pr_a p)
-        (fun pr pr_a p ls (_:unit) => ls ~~ Exists r :@ LinkedList, 
-            llist r (filter_model ls a) * pr --> node pr_a r)
-        (fun self pr pr_a p ls =>
-          IfNull p As p'
-          Then {{Return tt}}
-          Else nde <- !p';
-               if eq_a (data nde) a then 
-                 pr ::=  node pr_a (next nde);; 
-                 Free p';;
-                 {{self pr pr_a (next nde) (ls ~~~ tail ls) <@> 
-                   (ls ~~ [head ls = Some (data nde)] * [p = Some p'])}}
-               else 
-                 {{self p' (data nde) (next nde) (ls ~~~ tail ls) <@> 
-                   (ls ~~ [head ls = Some (data nde)] * [p = Some p'] * 
-                     pr --> node pr_a p)}}
-      ) pr' pr_a' p' ls');
-    q.
-  Qed.
+      STsep (ls' ~~ llist' p' ls' * pr' --> node pr_a' p')
+            (fun (_:unit) => ls' ~~ Exists r :@ LinkedList', 
+                llist' r (filter_model eq_a ls' a) * pr' --> node pr_a' r).
+      refine (fun pr' p' pr_a' a ls' =>
+        Fix4 (fun pr pr_a p ls => ls ~~ llist' p ls * pr --> node pr_a p)
+             (fun pr pr_a p ls (_:unit) => ls ~~ Exists r :@ LinkedList', 
+               llist' r (filter_model eq_a ls a) * pr --> node pr_a r)
+             (fun self pr pr_a p ls =>
+               IfNull p As p' Then
+                 {{Return tt}}
+               Else
+                 nde <- !p';
+                 if eq_a (data nde) a then 
+                   pr ::=  node pr_a (next nde);; 
+                   Free p';;
+                   {{ self pr pr_a (next nde) (ls ~~~ tail ls) <@> 
+                        (ls ~~ [head ls = Some (data nde)] * [p = Some p']) }}
+                 else 
+                   {{ self p' (data nde) (next nde) (ls ~~~ tail ls) <@> 
+                        (ls ~~ [head ls = Some (data nde)] * [p = Some p'] * pr --> node pr_a p) }}
+             ) pr' pr_a' p' ls');
+      try clear self; q.
+    Qed.
   
-  Definition filter : forall (p : LinkedList) (a : t) (ls : [list t]),
-    STsep (ls ~~ llist p ls)
-          (fun r:LinkedList => ls ~~ llist r (filter_model ls a)).
-    intros;
-    refine (
-      IfNull p As p' Then 
-        {{Return p}}
-      Else
-        nde <- !p';
-        {{filter' p' (next nde) (data nde) a (ls ~~~ tail ls) <@> 
-            (ls ~~ [head ls = Some (data nde)])}};;
-        if eq_a (data nde) a then
+    Definition filter' : forall (p : LinkedList') (a : t) (ls : [list t]),
+      STsep (ls ~~ llist' p ls)
+            (fun r:LinkedList' => ls ~~ llist' r (filter_model eq_a ls a)).
+      refine (fun p a ls =>
+        IfNull p As p' Then 
+          {{Return p}}
+        Else
           nde <- !p';
-          Free p';;
-          {{Return (next nde)}}
-        else
-          {{Return p}});
-    q.
-  Qed.
+          {{ filter_help' p' (next nde) (data nde) a (ls ~~~ tail ls) <@> 
+              (ls ~~ [head ls = Some (data nde)]) }};;
+          if eq_a (data nde) a then
+            nde <- !p';
+            Free p';;
+            {{ Return (next nde) }}
+          else
+            {{ Return p }});
+      q.
+    Qed.
 
-End Remove.
+  End Remove.
+
+  Definition HeapLinkedListSeg := mkList
+    llseg' empty' cons' single' freeList' freeHead' append' copy'
+    insertAt' elements' llseg'_unfold_nil removeFirst' filter' process' 
+    foldr_f' foldl' foldr'.
 
 End HeapLinkedList.
+
+  
