examples/servers/GradebookApp.v
@@ -1,0 +1,129 @@
+Require Import Ynot Basis IO.
+Require Import List.
+Require Import Parsers.
+Require Import GradebookModel AppServer.
+
+(* An implementation must specify the following: *)
+Module Type GradebookImpl.
+  Open Scope hprop_scope.
+  Parameter T: Set.
+  Parameter rep : forall (t: T) (m: (Config * list (ID * (list Grade)))), hprop.
+  Parameter exec' : forall (t : T) (q : ParseCommand) (m : [(Config * list (ID * (list Grade)))]),
+    STsep (m ~~ rep t m * [store_inv (snd m) (fst m) = true] ) 
+    (fun r : Status => m ~~ [r  = fst (mutate (compileCommand (fst m) q) m)] *  
+                            rep t (snd (mutate (compileCommand (fst m) q) m)) * 
+                            [store_inv (snd m) (fst m) = true] ).
+  Parameter init :
+    STsep (__)
+          (fun tm : T * [(Config * list (ID * (list Grade)))] => 
+            hprop_unpack (snd tm) (fun m => rep (fst tm) m * 
+              ([store_inv (snd m) (fst m) = true]))).
+
+  Parameter cleanup : forall (t : T) (m : [(Config * list (ID * (list Grade)))]),
+    STsep (m ~~ rep t m * [store_inv (snd m) (fst m) = true])
+          (fun _:unit => __).
+
+End GradebookImpl.
+
+Module Type GradebookType.
+  Definition Q : Set := ParseCommand.
+  Definition RR : Set := Status.
+
+  Definition M : Set := (Config * list (ID * (list Grade)))%type. 
+  Parameter T : Set.
+
+  Parameter rep : T -> M -> hprop.
+
+  Parameter func : Q -> M -> (RR * M).
+  Parameter AppIO : Q -> M -> RR -> M -> Trace.
+
+  Parameter I : M -> Prop.
+
+  Parameter func_preserves_I : forall q m, I m -> I (snd (func q m)).
+
+  Open Local Scope hprop_scope.
+  Parameter exec : forall (t : T) (q : Q) (m : [M]) (tr : [Trace]),
+    STsep (tr ~~ m ~~ rep t m  * traced tr * [I m]  ) 
+          (fun r : RR => tr ~~ m ~~ 
+             let m' := snd (func q m)
+             in  [r = fst (func q m)] * rep t m' * [I m'] *
+                 traced (AppIO q m r m' ++ tr)  ).
+  
+  Parameter init :
+    STsep (__)
+          (fun tm : T * [M] => hprop_unpack (snd tm) (fun m => rep (fst tm) m * [I m])).
+
+  Parameter cleanup : forall (t : T) (m : [M]),
+    STsep (m ~~ rep t m * [I m])
+          (fun _:unit => __).
+
+End GradebookType.
+
+
+(* From that, we can build a runnable app. *)
+Module Gradebook (X: GradebookImpl) : GradebookType.
+  Export X. 
+
+  Definition Q : Set := ParseCommand.
+  Definition M : Set := (Config * list (ID * (list Grade)))%type. 
+  Definition T := T. 
+  Definition RR : Set := Status.
+
+  Definition rep := rep.
+
+  Definition func (q: Q) (m: M) : (RR * M).
+    unfold Q. unfold M. unfold RR. intros q m. exact (mutate (compileCommand (fst m) q) m). 
+  Defined.
+  Definition AppIO (_:Q) (_:M) (_:RR) (_:M) := (@nil Action).
+
+  Open Scope hprop_scope.
+  Open Scope stsepi_scope.
+
+  Definition exec' := exec'.  
+
+  Open Scope string_scope. 
+
+  Definition I m : Prop := store_inv (snd m) (fst m) = true .
+
+  Definition func_preserves_I : forall q m, I m -> I (snd (func q m)).
+   intros. unfold I in *. unfold func. destruct m. simpl in H. unfold store_inv in *. 
+   assert (store_inv1 l c = true /\ total_dec (students c) l = true).
+   destruct (store_inv1 l c). destruct (total_dec (students c) l). 
+   firstorder. simpl in H. discriminate.
+   simpl in H. discriminate. 
+   simpl.
+   Ltac exhaustive solver :=
+    simpl; 
+    repeat (match goal with 
+              | [ |- context [ if ?X then _ else _ ] ] => case_eq X
+              | [ |- context [ match ?X with | Some _ => _ | None => _ end ] ] => case_eq X
+              | [ |- context [ match ?X with | SetGrade _ _ _ _ _ => _ | GetGrade _ _ _ _ => _ | Average _ _ _ => _ end ] ] => case_eq X
+            end; intros; simpl; try solver).
+   Hint Resolve insert_preserves_inv insert_preserves_total_dec insert_preserves_noduples.
+   all; each; exhaustive ltac:(auto).
+ Qed.
+
+ 
+ Definition exec (t : T) (q : Q) (m : [M]) (tr : [Trace]) :
+   STsep (tr ~~ m ~~ rep t m  * traced tr * [I m]  ) 
+         (fun r : RR => tr ~~ m ~~ 
+           let m' := snd (func q m)
+           in  [r = fst (func q m)] * rep t m' * [I m'] *
+               traced (AppIO q m r m' ++ tr)  ).
+   intros; refine ( 
+     r <- exec' t q m <@> (tr ~~ traced tr) ;
+     {{ Return r }}).
+   solve [ sep fail auto ].
+   solve [ sep fail auto ].
+   solve [ sep fail auto ].
+   solve [ sep fail auto; pose (i := func_preserves_I q x0); unfold I in *; sep fail auto ].
+ Qed. 
+
+Definition init := init.
+
+Definition cleanup := cleanup.
+
+End Gradebook.
+
+Require Export List.
+Require Export GradebookModel AppServer.
