examples/servers/GradebookInterface.v
@@ -1,0 +1,166 @@
+Require Import Ynot Basis.
+Require Import Ascii String Stream.
+Require Import Parsec Charset.
+Require Import Arith.
+Require Import GradebookApp.
+Require Import Parsers.
+
+Set Implicit Arguments.
+
+Module GradebookParser.
+  Import ParsecCombinators.Combinators.
+  Import ParsecNotation.
+
+(**
+  (* A grammar for digits *)  
+  Definition is_digit(c:ascii):bool := 
+    if le_lt_dec (nat_of_ascii "0"%char) (nat_of_ascii c) then
+      (if le_lt_dec (nat_of_ascii c) (nat_of_ascii "9"%char) then true else false)
+    else false.
+
+  Definition digit : Term ascii  := gsatisfy is_digit.
+
+  (* A parser for digits *)
+  Definition digit_p : parser_t digit := satisfy is_digit.
+
+  (** grammar for letters **)
+  Definition is_alpha(c:ascii) : bool :=
+    if le_lt_dec (nat_of_ascii "a"%char) (nat_of_ascii c) then 
+      (if le_lt_dec (nat_of_ascii c) (nat_of_ascii "z"%char) then true else false)
+    else false.
+
+  Definition is_Alpha(c:ascii) : bool :=
+    if le_lt_dec (nat_of_ascii "A"%char) (nat_of_ascii c) then 
+      (if le_lt_dec (nat_of_ascii c) (nat_of_ascii "Z"%char) then true else false)
+    else false.
+
+  Definition is_letter(c:ascii) : bool := if (is_alpha c) then true else (is_Alpha c).
+
+  Definition letter : Term ascii := gsatisfy is_letter.
+  Definition letter_p : parser_t letter := satisfy is_letter.
+
+
+  Definition tab : ascii := ascii_of_nat 9.
+  Definition cr : ascii := ascii_of_nat 13.
+  Definition lf : ascii := ascii_of_nat 10.
+
+  Definition crlf : Term unit :=
+    fun _ => (# cr ^ #lf @ (fun _ => tt))%grammar.
+  
+  Definition crlf_p : parser_t crlf.
+    refine ((# cr ^ #lf @ (fun _ => tt)))%parser.
+  Qed.    
+**)
+
+  Export GradebookModel.
+
+  Definition id : Term AsciiCharset string := str.
+  Definition id_p : parser_t id := str_p.
+
+  Definition pass : Term AsciiCharset string := str.
+  Definition pass_p : parser_t pass := str_p.
+
+  Definition assign : Term AsciiCharset string := str.
+  Definition assign_p : parser_t assign := str_p.
+
+  Definition grade : Term AsciiCharset Grade := number.
+  Definition grade_p : parser_t grade := number_p.
+
+  Definition section : Term AsciiCharset Section :=
+    fun var => (digit _ @ (fun v => nat_of_ascii v - nat_of_ascii "0"%char))%grammar.
+  Definition section_p : parser_t section :=
+    (digit_p @ (fun v => nat_of_ascii v - nat_of_ascii "0"%char))%parser.
+
+  Definition id_pass : Term AsciiCharset (string * string) :=
+    fun var => 
+      (#"[" ^ id _ ^ ws _ ^ pass _ ^ #"]" @ (fun x => (fst (snd x), fst (snd (snd (snd x))))))%grammar.
+  Definition id_pass_p : parser_t id_pass :=
+    (#"[" ^ id_p ^ ws_p ^ pass_p ^ #"]" @ (fun x => (fst (snd x), fst (snd (snd (snd x))))))%parser.
+
+
+  Definition CommandGrammar : Term AsciiCharset ParseCommand := 
+    fun var =>
+      (    #"G" ^ #"E" ^ #"T" ^ ws _ ^ id_pass _ ^ ws _ ^ id _ ^ ws _ ^ assign _ @ 
+             (fun x => 
+               let up := (fst (snd (snd (snd (snd x))))) in
+               let id := (fst (snd (snd (snd (snd (snd (snd x))))))) in
+               let assign := (snd (snd (snd (snd (snd (snd (snd (snd x)))))))) in
+               GetGrade' (fst up) (snd up) id assign)
+       ||| #"S" ^ #"E" ^ #"T" ^ ws _ ^ id_pass _ ^ ws _ ^ id _ ^ ws _ ^ assign _ ^ ws _ ^ grade _ @ 
+             (fun x => 
+               let up := (fst (snd (snd (snd (snd x))))) in
+               let id := (fst (snd (snd (snd (snd (snd (snd x))))))) in
+               let assign := (fst (snd (snd (snd (snd (snd (snd (snd (snd x))))))))) in
+               let gr := snd (snd (snd (snd (snd (snd (snd (snd (snd (snd x))))))))) in
+               SetGrade' (fst up) (snd up) id assign gr)
+       ||| #"A" ^ #"V" ^ #"G" ^ ws _ ^ id_pass _ ^ ws _ ^ assign _ @ 
+             (fun x => 
+               let up := (fst (snd (snd (snd (snd x))))) in
+               let assign := (snd (snd (snd (snd (snd (snd x)))))) in
+               Average' (fst up) (snd up) assign))%grammar.
+
+  Definition CommandParser : parser_t CommandGrammar :=
+      (    #"G" ^ #"E" ^ #"T" ^ ws_p ^ id_pass_p ^ ws_p ^ id_p ^ ws_p ^ assign_p @ 
+             (fun x => 
+               let up := (fst (snd (snd (snd (snd x))))) in
+               let id := (fst (snd (snd (snd (snd (snd (snd x))))))) in
+               let assign := (snd (snd (snd (snd (snd (snd (snd (snd x)))))))) in
+               GetGrade' (fst up) (snd up) id assign)
+       ||| #"S" ^ #"E" ^ #"T" ^ ws_p ^ id_pass_p ^ ws_p ^ id_p ^ ws_p ^ assign_p ^ ws_p ^ grade_p @ 
+             (fun x => 
+               let up := (fst (snd (snd (snd (snd x))))) in
+               let id := (fst (snd (snd (snd (snd (snd (snd x))))))) in
+               let assign := (fst (snd (snd (snd (snd (snd (snd (snd (snd x))))))))) in
+               let gr := snd (snd (snd (snd (snd (snd (snd (snd (snd (snd x))))))))) in
+               SetGrade' (fst up) (snd up) id assign gr)
+       ||| #"A" ^ #"V" ^ #"G" ^ ws_p ^ id_pass_p ^ ws_p ^ assign_p @ 
+             (fun x => 
+               let up := (fst (snd (snd (snd (snd x))))) in
+               let assign := (snd (snd (snd (snd (snd (snd x)))))) in
+               Average' (fst up) (snd up) assign))%parser.
+
+End GradebookParser.
+
+
+Module HttpGradebookInterface (AP : GradebookType) : AppInterface with Module A := AP.
+  Module A := AP.
+
+  Definition grammar := GradebookParser.CommandGrammar.
+  Definition parser  := GradebookParser.CommandParser.
+
+  Open Local Scope string_scope.
+  Export Basis.
+
+  Definition header : list ascii := str2la (
+(*    "<?xml version=""1.0""?>" ++  *)
+    "<!DOCTYPE HTML PUBLIC ""-//W3C//DTD HTML 4.01//EN"" ""http://www.w3.org/TR/html4/strict.dtd"">" ++
+    "<html>" ++
+    " <head>" ++
+    "  <title>Course Grade Server</title>" ++
+    " </head>" ++
+    " <body>" ++
+    "  <form action=""http://127.0.0.1:8081"" method=""GET"" target=""_self"">" ++
+    "   Query <input type=""text"" name=""q"" size=""25"" maxlength=""40"" /> <input type=""submit"" />" ++
+    "  </form>" ++
+    "  <br />"). 
+
+  Definition footer : list ascii := str2la (
+    " </body>" ++
+    "</html>").
+
+  Definition printer (res : Status) : list ascii :=
+    List.app header
+    (List.app
+      match res with
+        | ERR_NOTPRIVATE => str2la "<b color=""red"">Error:</b> Not Private"
+        | ERR_BADGRADE => str2la "<b color=""red"">Error:</b> Bad Grade"
+        | ERR_NOINV => str2la "<b color=""red"">Error:</b> No Invariant"
+        | OK => str2la "<b color=""green"">Success!</b>"
+        | RET x => List.app (str2la "<b color=""green"">Result:</b> ") (ntos 3 x nil)
+      end
+      footer).
+  
+  Definition err (_ : consumed_t) := 
+    List.app header (List.app (str2la "<b color=""red"">Error:</b> Malformed query") footer).
+
+End HttpGradebookInterface.
