examples/servers/GradebookRefImpl.v
@@ -1,0 +1,44 @@
+Require Import Ynot RSep.
+Require Import GradebookApp GradebookModel AppServer.
+
+(* Reference to a logical model. *)
+Module GradebookRefImpl : GradebookImpl.
+  Open Scope hprop_scope.
+  Open Scope stsepi_scope.
+
+  Definition T := ptr.
+
+  Definition rep (t: T) (m: (Config * list (ID * (list Grade)))) : hprop := ( t --> m ).
+
+  Definition exec' : forall (t : T) (q : ParseCommand) (m : [(Config * list (ID * (list Grade)))]),
+    STsep (m ~~ rep t m * [store_inv (snd m) (fst m) = true] ) 
+          (fun r : Status => m ~~ [r  = fst (mutate (compileCommand (fst m) q) m)] *  rep t (snd (mutate (compileCommand (fst m) q) m)) * 
+            [store_inv (snd m) (fst m) = true] ).
+    intros. refine ( x <- ! t ;
+                     let res := mutate (compileCommand (fst x) q) x in
+                     t ::= snd res ;;
+                     {{ Return (fst res) }} ); unfold rep;
+    try solve [ sep fail auto | unfold res; rsep fail auto; subst; sep fail auto].
+  Qed.
+
+  Export ExampleConfig.
+  Definition init :
+    STsep (__)
+          (fun tm : T * [(Config * list (ID * (list Grade)))] => hprop_unpack (snd tm) 
+            (fun m => rep (fst tm) m * [store_inv (snd m) (fst m) = true] )).
+    unfold rep; refine ( x <- New test_model ;
+                         {{ Return (x, inhabits test_model) }} ); pose test_cfg_inv;
+    sep fail auto. 
+  Qed.
+
+  Definition cleanup (t : T) (m : [(Config * list (ID * (list Grade)))]) :
+    STsep (m ~~ rep t m * [store_inv (snd m) (fst m) = true])
+          (fun _:unit => __).
+    intros. refine {{Free t}}.
+    unfold rep. sep fail auto.
+    rsep fail auto.
+  Qed.
+
+End GradebookRefImpl. 
+
+Module theApp : App := GradebookApp.Gradebook (GradebookRefImpl).
