examples/servers/HttpParsec.v
@@ -1,0 +1,58 @@
+Require Import Ynot.
+Require Import Ascii.
+Require Import Stream.
+Require Import Parsec Charset ParsecCombinators.
+Require Import Arith.
+Require Import String.
+
+Set Implicit Arguments.
+
+Module Http.
+  Import Combinators.
+  Import ParsecNotation.
+
+  Definition crlf : Term AsciiCharset unit :=
+    fun _ => (# cr ^ #lf @ (fun _ => tt))%grammar.
+  
+  Definition crlf_p : parser_t crlf.
+    refine ((# cr ^ #lf @ (fun _ => tt)))%parser.
+  Qed.    
+
+  Definition HTTP : Term AsciiCharset string := 
+    fun var => 
+    (#"G" ^ #"E" ^ #"T" ^ ws _ ^ str _ ^ ws _ ^ #"H" ^ #"T" ^ #"T" ^ #"P" ^ #"/" ^ # "1" ^ #"." ^ digit _ ^ crlf _ ^ crlf _ @ (fun x => fst (snd (snd (snd (snd x))))))%grammar.
+
+  Definition HTTP_p : parser_t HTTP :=
+    (#"G" ^ #"E" ^ #"T" ^ ws_p ^ str_p ^ ws_p ^ #"H" ^ #"T" ^ #"T" ^ #"P" ^ #"/" ^ # "1" ^ #"." ^ digit_p ^ crlf_p ^ crlf_p @ (fun x => fst (snd (snd (snd (snd x))))))%parser.
+
+End Http.
+
+Open Local Scope stsepi_scope.
+Require Import Basis.
+
+Require Import GradebookInterface.
+
+Definition parse_test : forall (input : string),
+  STsep (__) 
+        (fun _ : option string (*nat * ((method * string * (nat * nat)) * (list (string * string)) * string)*) => __)%hprop.
+  intros; refine (
+     printStringLn' (str2la input) ;;
+     is <- STRING_INSTREAM.instream_of_list_ascii (str2la input) ;
+     (* parse <- http_parse is (inhabits 0) ; *)
+     parse <- GradebookInterface.GradebookParser.CommandParser is (inhabits 0) ;
+     INSTREAM.close is ;;
+     {{Return (match parse with 
+                 | ERROR _ _ => None
+                 | OKAY _ _ q => Some "good"%string
+               end)}}).
+  sep fail auto.
+  sep fail auto.
+  sep fail auto.
+  sep fail auto.
+  sep fail auto.
+  sep fail auto.
+  unfold ans_str_correct, okaystr,errorstr,okay,error; destruct parse; sep fail auto.
+  sep fail auto.
+  sep fail auto.
+  sep fail auto.
+Qed.
