examples/servers/HttpParser.v
@@ -1,0 +1,214 @@
+Require Import Ynot.
+Require Import Charset Packrat.
+Require Import List Ascii String.
+
+Set Implicit Arguments.
+
+(**
+       URI            = ( absoluteURI | relativeURI ) [ "#" fragment ]
+
+       absoluteURI    = scheme ":" *( uchar | reserved )
+
+       relativeURI    = net_path | abs_path | rel_path
+
+       net_path       = "//" net_loc [ abs_path ]
+       abs_path       = "/" rel_path
+       rel_path       = [ path ] [ ";" params ] [ "?" query ]
+
+       path           = fsegment *( "/" segment )
+       fsegment       = 1*pchar
+       segment        = *pchar
+
+       params         = param *( ";" param )
+       param          = *( pchar | "/" )
+
+       scheme         = 1*( ALPHA | DIGIT | "+" | "-" | "." )
+       net_loc        = *( pchar | ";" | "?" )
+       query|fragment = *( uchar | reserved )
+
+       pchar          = uchar | ":" | "@" | "&" | "=" | "+"
+       uchar          = unreserved | escape
+       unreserved     = ALPHA | DIGIT | safe | extra | national
+
+       escape         = "%" HEX HEX
+       reserved       = ";" | "/" | "?" | ":" | "@" | "&" | "=" | "+"
+       extra          = "!" | "*" | "'" | "(" | ")" | ","
+       safe           = "$" | "-" | "_" | "."
+       unsafe         = CTL | SP | <""> | "#" | "%" | "<" | ">"
+       national       = <any OCTET excluding ALPHA, DIGIT,
+                        reserved, extra, safe, and unsafe>
+**)
+Import Packrat.
+
+
+Definition alpha := Terminal AsciiCharset (ARange "a" "z").
+Definition Alpha := Terminal AsciiCharset (ARange "A" "Z").
+Definition digit := Terminal AsciiCharset (ARange "0" "9").
+
+Section Combinators.
+  Variable base_ty : Set.
+  Variable base_ty_denote : base_ty -> Set.
+  Definition ty := @ty base_ty.
+  Definition tyDenote : ty -> Set := @tyDenote ascii base_ty base_ty_denote.
+  Definition term := @term ascii.
+
+  Definition many ctx (T S : ty) (t: tyDenote T) (f : tyDenote S -> tyDenote T -> tyDenote T)
+    (prin : term _ ctx S) (rec : term _ ctx T) : term _ ctx T :=
+    (Alt (Map _ (fun a : tyDenote (Prod S T) => f (fst a) (snd a)) (Seq prin rec))
+         (Map _ (fun _ => t) (@Epsilon ascii base_ty base_ty_denote ctx))).
+
+  Definition many1 ctx (T S : ty) (t: tyDenote S -> tyDenote T) 
+    (f : tyDenote S -> tyDenote T -> tyDenote T)
+    (prin : term _ ctx S) (rec : term _ ctx T) : term _ ctx T :=
+    (Alt (Map _ (fun a:tyDenote (Prod S T) => f (fst a) (snd a)) (Seq prin rec))
+         (Map _ (t) (prin))).
+End Combinators.
+
+Set Printing All.
+Definition manyStr ctx : term (fun _:unit => string) ctx (Char unit) -> term (fun _:unit => string) ctx (Base tt) -> term (fun _:unit => string) ctx (Base tt) :=
+  @many unit (fun _:unit => string) ctx (Base tt) (Char unit) EmptyString String.
+
+Definition many1Str ctx : term (fun _:unit => string) ctx (Char unit) -> term (fun _:unit => string) ctx (Base tt) -> term (fun _:unit => string) ctx (Base tt) :=
+  @many1 unit (fun _:unit => string) ctx (Base tt) (Char unit) (fun a:tyDenote (fun _:unit => string) (Char unit) => String a EmptyString) String.
+
+Definition cat ctx (c : ascii) (s : term ctx string) : term ctx string :=
+  Map _ (fun a => String (fst a) (snd a)) (Seq (Lit ctx c) s).
+
+Definition optional ctx (T : Set) (t : T) (c : term ctx T) : term ctx T :=
+  Alt c (Map (fun _ => t) (Epsilon _)).
+
+Fixpoint litString ctx (T : Set) (t : T) (s : string) : term ctx T :=
+  match s with
+    | EmptyString => (Map (fun _ => t) (Epsilon ctx))
+    | String a r => (Map (fun _ => t) (Seq (Lit _ a) (litString ctx t r)))
+  end.
+
+(* Notation "# c" := (AsciiParser.Lit _ c%char) (at level 1) : grammar_scope. *)
+Notation "## c" := (AsciiParser.LitClass _ c%char) (at level 1) : grammar_scope.
+Notation "e1 ^^ e2" := (AsciiParser.Seq e1 e2) (right associativity, at level 30) : grammar_scope.
+Notation "e @@ f" := (AsciiParser.Map f e) (left associativity, at level 78) : grammar_scope.
+Notation "e1 || e2" := (AsciiParser.Alt e1 e2) (right associativity, at level 79) : grammar_scope.
+
+Open Local Scope grammar_scope.
+
+Fixpoint enum ctx (T : Set) (t':T) (t : list (string * T)) : term ctx T :=
+  match t with
+    | nil => ## (Group nil) @@ (fun _ => t') (** This is essentially the error production **)
+    | (str,v) :: r => (litString _ v str) || enum ctx t' r
+  end.
+
+Definition crlf ctx : term ctx unit := (Lit _ (ascii_of_nat 13)) ^^ (Lit _ (ascii_of_nat 10)) @@ (fun _ => tt).
+Definition sp ctx : term ctx unit := (Lit _ " "%char) @@ (fun _ => tt
+Inductive method : Set :=
+| GET : method | POST : method | HEAD : method.
+
+Definition HTTP_ctx := 
+       (nat ::
+        ascii :: ascii :: ascii :: ascii ::
+        ascii :: ascii :: ascii ::
+        string ::
+        string :: string ::
+        string :: string :: string ::
+        string :: string :: string ::
+        method :: (nat * nat) :: (method * string * (nat * nat)) ::
+        string :: string :: (string * string) :: list (string * string) ::
+        string :: 
+        string :: ((method * string * (nat * nat)) * (list (string * string)) * string) :: nil)%type.
+
+Definition HTTP_env :=
+  gfix HTTP_ctx
+  (fun number
+       unsafe safe extra reserved
+       unreserved uchar pchar
+       fragment
+       param params
+       segment fsegment path
+       rel_path abs_path request_uri
+       method http_ver request_line
+       header_seg header_value header headers
+       body
+       simple_req request =>
+    (* 0 *)
+    (## digit @@ (fun t => nat_of_ascii t - nat_of_ascii "0"%char),
+
+    (* 1 *)
+    (## (Group ("?" :: " " :: """" :: "#" :: "%" :: "<" :: ">" :: nil)),
+    (## (Group ("$" :: "-" :: "_" :: "." :: nil)),
+    (## (Group ("!" :: "*" :: "'" :: "(" :: ")" :: "," :: nil)),
+    (## (Group (";" :: "/" :: "?" :: ":" :: "@" :: "&" :: "=" :: "+" :: nil)),
+
+    (* 5 *)
+    ((## (Union (Union alpha Alpha) digit)) || safe || extra,
+    (unreserved || reserved,
+    (uchar || (## (Group (":" :: "@" :: "&" :: "=" :: "+" :: nil))),
+
+    (* 8 *)
+    (manyStr (uchar || reserved || (Lit _ "%"%char)) fragment,
+
+    (* 9 *)
+    (manyStr (pchar || (Lit _ "/"%char)) param,
+    (Map (fun a => String.append (fst a) (snd a))
+         (param ^^ (many EmptyString (String.append) (cat ";" param) params)),
+
+    (* 11 *)
+    (manyStr pchar segment,
+    (many1Str pchar fsegment,
+    (Map (fun a => append (fst a) (snd a)) (fsegment ^^ (cat "/" segment)),
+
+    (* 14 *)
+    (Map (fun a => append (fst a) (append (fst (snd a)) (snd (snd a))))
+         ((optional EmptyString  path) ^^
+           ((optional EmptyString (cat ";" params)) ^^
+             (optional EmptyString (cat "?" fragment)))), 
+(*    (segment, *)
+    (cat "/" rel_path,
+    (abs_path,
+
+    (* 17 *)
+    (enum _ GET (("GET", GET) :: ("POST", POST) :: ("HEAD", HEAD) :: nil)%string,
+    ((litString _ tt "HTTP/") ^^ number ^^ (Lit _ "."%char) ^^ number @@ (fun t => (fst (snd t), snd (snd (snd t)))),
+    (method ^^ (Lit _ " "%char) ^^ request_uri ^^ (Lit _ " "%char) ^^ http_ver ^^ crlf _ @@ (fun t => (fst t, fst (snd (snd t)), fst (snd (snd (snd (snd t)))))),
+
+    (* 20 *)
+    (many1Str (unreserved) header_seg,
+    (many1Str (unreserved || extra || reserved || unsafe || (Lit _ " "%char)) header_value,
+    (header_seg ^^ (litString _ tt ": ") ^^ header_value ^^ crlf _ @@ (fun t => (fst t, fst (snd (snd t)))),
+    (many nil (fun a b => a :: b) header headers,
+
+    (* 24 *)
+    (manyStr (## All) body,
+
+    (* 25 *)
+    ((litString _ (EmptyString) "GET") ^^ (Lit _ " "%char) ^^ rel_path ^^ crlf _ @@ (fun t => fst (snd (snd t))),
+    (request_line ^^ headers ^^ crlf _ ^^ body @@ (fun t => (fst t, fst (snd t), snd (snd (snd t)))),
+
+      tt)))))))))))))))))))))))))))
+  ).
+
+Open Local Scope hprop_scope.
+
+Definition HTTP_simple_correct
+    (ins : Stream.INSTREAM.instream_t char) (n : [nat]) (a : option (nat * string)) :=
+  ans_correct HTTP_env ins n (Var HTTP_ctx 25) a.
+
+Definition simple_http_parse' :=
+  AsciiParser.mkparser (HTTP_env) (AsciiParser.Var _ 25).
+
+Definition simple_http_parse : forall (ins : Stream.INSTREAM.instream_t char) (n : [nat]),
+  STsep (n ~~ Stream.INSTREAM.rep ins n)
+        (fun a : option (nat * string) =>
+          HTTP_simple_correct ins n a * rep_ans ins n a) :=
+  simple_http_parse'.
+
+Definition HTTP_correct
+    (ins : Stream.INSTREAM.instream_t char) (n : [nat]) 
+    (a : option (nat * ((method * string * (nat * nat)) * list (string * string) * string))) := 
+  ans_correct HTTP_env ins n (Var HTTP_ctx 26) a.
+
+Definition http_parse' := AsciiParser.mkparser (HTTP_env) (AsciiParser.Var _ 26).
+
+Definition http_parse : forall (ins : Stream.INSTREAM.instream_t char) (n : [nat]),
+  STsep (n ~~ Stream.INSTREAM.rep ins n)
+        (fun a : option (nat * ((method * string * (nat * nat)) * (list (string * string)) * string)) =>
+          HTTP_correct ins n a * rep_ans ins n a) :=
+  http_parse'.
