examples/servers/HttpTest.v
@@ -1,0 +1,23 @@
+Require Import Ynot Basis.
+Require Import List Ascii String.
+Require Import RSep.
+Require Import HttpParser.
+Require Import Stream.
+
+
+
+Open Local Scope stsepi_scope.
+Open Local Scope hprop_scope.
+
+Ltac s := unfold PackRatParser.AsciiParser.CH.char, PackRatParser.AsciiCharset.char,PackRatParser.AsciiParser.rep_ans, HTTP_correct,PackRatParser.AsciiParser.ans_correct in *; rsep fail auto.
+
+Definition parse_test : forall (str : string),
+  STsep (__) 
+        (fun _ : option (nat * ((method * string * (nat * nat)) * (list (string * string)) * string)) => __).
+  intros; refine (
+     is <- STRING_INSTREAM.instream_of_list_ascii (str2la str) ;
+     parse <- http_parse is (inhabits 0) ;
+     INSTREAM.close is ;;
+     {{Return parse}});
+  solve [ s | destruct parse; sep fail auto ].
+Qed.
