examples/servers/Mapping2.v
@@ -1,0 +1,180 @@
+Require Import GradebookModel. (* change this module name or move to here *)
+Require Import List.
+
+Set Implicit Arguments.
+
+Module Config.
+  (* privacy respecting queries can probably stay the same *)
+  Definition P (cfg: Config) (q: Command) := True.
+  (* likewise with correct queries *)
+  Definition E (cfg: Config) (q: Command) := True. 
+  (* todo add definition of privacy and wellformedness of q *)
+  Parameter P_dec : forall cfg q, {P cfg q} + {~P cfg q}. (* privacy *)
+  Parameter E_dec : forall cfg q, {E cfg q} + {~E cfg q}. (* valid query *)
+End Config.
+
+Module Type Model.
+  Export Config.
+  Parameter M : Type.
+  Parameter I : Config -> M -> Prop.
+  Parameter mutate : forall (cfg: Config) (q: Command) (m: M), (Status * M).
+  Parameter pres_I : forall cfg q m,
+    I cfg (snd (mutate cfg q m)).
+End Model.
+
+Require Import Ynot.
+Module Type Impl (X: Model).
+ Export X.
+  Parameter T: Set.
+  Parameter rep : forall (t: T) (m: M), hprop.
+
+  Open Local Scope hprop_scope.
+  Parameter imp_mutate : forall cfg t q (m: [M]),
+    STsep (m ~~ rep t m * [I cfg m] * [P cfg q] * [E cfg q]) 
+          (fun r : Status => m ~~ let (r', m') := (mutate cfg q m)
+                                  in  [r' = r] * rep t m'). 
+End Impl.
+ 
+(* our spec is a distinguished model *) 
+Module Spec : Model.
+ Export Config.
+   Definition  M := ID -> Assignment -> option Grade. 
+   
+   Definition  I : Config -> M -> Prop. 
+   Admitted.
+  
+  Parameter mutate : forall (cfg: Config) (q: Command) (m: M), (Status * M).
+
+    Theorem pres_I : forall cfg q m,
+    I cfg (snd (mutate cfg q m)).
+    Admitted.
+End Spec.
+
+(* The model of the imperative implementation *)
+Module TupleModel : Model.
+ Export Config.
+   Definition  M := ID -> Assignment -> option Grade. 
+   
+   Definition  I : Config -> M -> Prop. 
+   Admitted.
+  
+  Parameter mutate : forall (cfg: Config) (q: Command) (m: M), (Status * M).
+
+    Theorem pres_I : forall cfg q m,
+    I cfg (snd (mutate cfg q m)).
+    Admitted.
+End TupleModel.
+
+(* equivalences of models *)
+Module Type ModelIso.
+  Export Config.
+  Declare Module S : Model.
+  Declare Module T : Model.
+
+  Parameter f : forall cfg, sigT (S.I cfg) -> sigT (T.I cfg).
+  Parameter g : forall cfg, sigT (T.I cfg) -> sigT (S.I cfg).
+
+  (* we probably don't want 
+  Parameter Correct : forall cfg t, f (cfg:=cfg)(g t) = t. *)
+  
+  Parameter Correct : forall cfg t, 
+   projT1 (f (g (cfg:=cfg) t)) = projT1 t. 
+End ModelIso.
+
+Module CorrectRefl (X: Model) : ModelIso with Module S := X 
+                                         with Module T := X.
+  Export Config.
+  Module S := X.
+  Module T := X.
+
+  Definition f cfg (x: sigT (S.I cfg)) := x.
+  Definition g cfg (y: sigT (T.I cfg)) := y. 
+
+  Theorem Correct : forall cfg t, 
+   projT1 (f (g (cfg:=cfg) t)) = projT1 t. 
+  Proof.
+    compute. intros. eauto. Qed.
+End CorrectRefl.
+
+(* todo the isomorphism of the models isn't quite implementation
+   correctness.  technically we need to take into account
+   the outer wrapping where the invariant is checked, where
+   privacy is checked, etc.  But that should be easy enough
+   to build off of this. *)
+Module ImplCorrect : ModelIso with Module S := Spec 
+                              with Module T := TupleModel.
+  Export Config.
+  Module S := Spec.
+  Module T := TupleModel.
+   
+  Definition f cfg (x: sigT (S.I cfg)) : sigT (T.I cfg). 
+  Admitted.
+  Definition g cfg (y: sigT (T.I cfg)) : sigT (S.I cfg). 
+  Admitted. 
+
+  Theorem Correct : forall cfg t, 
+   projT1 (f (g (cfg:=cfg) t)) = projT1 t. 
+  Proof.
+  Admitted.
+End ImplCorrect.
+
+(* we want to say that given a model and
+   an imperative realization of that model, that
+   we can build an app 
+Require Import AppServer.
+
+Module BuildApp (X: Model) (Y: Impl X) : App.
+ Module C := Y X.
+ Export C.
+ Open Local Scope hprop_scope.
+ Definition Q := Command.
+ Definition T : Set := (Config * C.T)%type.
+ Definition RR : Set := Status.
+ Definition M := (Config * X.M)%type.
+ Definition rep (t: T) (m: M) : hprop := [fst t = fst m] * C.rep (snd t) (snd m).
+ Definition I (m: M) : Prop := X.I (fst m) (snd m).
+ 
+ Definition func := X.mutate.
+
+End BuildApp.
+*)
+
+(* these wrappers may come in handy 
+   for above. *)
+Module WrapModel (X: Model).
+  Export X.
+
+  Definition wrap cfg q m (pf_I: I cfg m) :=
+    match P_dec cfg q with
+      | left  pf_P => match E_dec cfg q with
+                        | left  pf_E => mutate cfg q m  
+                        | right pf_badgrade => (ERR_BADGRADE, m) 
+                      end
+      | right pf_notpriv => (ERR_NOTPRIVATE, m)
+    end.
+End WrapModel.
+
+Require Import Ynot.
+Module WrapImpl (X: Model) (Y: Impl).
+ Module Z := Y X.
+ Export Z.
+ Module W := WrapModel X.
+ Export W.
+
+ Open Local Scope stsepi_scope.
+ Open Local Scope hprop_scope.
+ Definition imp_wrap cfg t q m : 
+  STsep (m ~~ rep t m * [I cfg m] * [P cfg q] * [E cfg q]) 
+   (fun r : Status => m ~~ Exists pf1 :@ I cfg m, 
+                           let (r', m') := (wrap q pf1 )
+                           in  [r' = r] * rep t m').
+ Admitted. 
+End WrapImpl.
+
+Require Import Store.
+
+(* And we need to do this as well
+Module StoreImpl (s: Store) : Impl TupleModel .
+ 
+End StoreImpl.
+*)
