examples/servers/PaperMapping2.v
@@ -1,0 +1,538 @@
+Require Import Ynot.
+Require Import GradebookModel. (* change this module name or move to here *)
+Require Import List.
+Require Import GradebookStoreImpl.
+Require Import Store.
+Require Import RSep.
+Require Import AppServer.
+Require Import IO.
+
+Set Implicit Arguments.
+
+Axiom shift : forall (P:Prop), (STsep [P] (fun pf : P => [P]))%hprop.
+
+(* ***************************************************************************************** *)
+(* Framework *)
+
+Module Type Model.
+  Parameter M : Config -> Type.
+  Parameter I : forall (cfg : Config), M cfg -> Prop.
+  Parameter mutate     : forall (cfg: Config) (m: M cfg)            (q: Command), (Status * M cfg).
+  Parameter PreservesI : forall (cfg: Config) (m: M cfg) (pfI: I m) (q: Command), I (snd (mutate m q)).
+End Model.
+
+(** A morphism between models **)
+Module Type ModelHomomorphism (* (S : Model) (T : Model) *).
+(* h (S.mutate x) = T.mutate (h x) *)
+  Declare Module S : Model.
+  Declare Module T : Model.
+
+  Parameter h : forall (cfg: Config), S.M cfg -> T.M cfg.
+   
+  Parameter InvPres : forall cfg (m: S.M cfg), S.I m -> T.I (h m).
+
+  Parameter ObserveEq : forall cfg (m: S.M cfg), S.I m ->
+    forall q, fst (S.mutate m q) = fst (T.mutate (h m) q).
+
+  Parameter StatePres : forall cfg (m: S.M cfg), S.I m ->
+    forall q, h (snd (S.mutate m q)) = snd (T.mutate  (h m) q).
+End ModelHomomorphism.
+
+(** This is an implementation of the S Model using the T Model **)
+Module Type Impl.
+  Declare Module Cert : ModelHomomorphism.
+  Module Spec := Cert.T.
+  Module Impl := Cert.S.
+
+  Parameter T   : Type.
+  Parameter rep : forall (cfg: Config) (t: T) (m: Impl.M cfg), hprop.
+
+  Open Local Scope hprop_scope.
+  (** This should be in terms of Impl **)
+  Parameter imp_mutate : forall cfg (t: T) q (m: [Impl.M cfg]),
+    STsep (m ~~ rep t m * [Impl.I m]) 
+          (fun r : Status => m ~~ let (r', m') := (Impl.mutate m q)
+                                  in  [r' = r] * rep t m' * [Impl.I m']).
+
+  Parameter init :
+    STsep (__)
+          (fun tm : T * sigT (fun cfg => inhabited (Impl.M cfg)) => hprop_unpack (projT2 (snd tm)) (fun m => rep (fst tm) m * [Impl.I m])).
+
+
+  Parameter cleanup : forall (cfg : Config) (t : T) (m : [Impl.M cfg]),
+    STsep (m ~~ rep t m * [Impl.I m])
+          (fun _:unit => __).
+
+End Impl.
+
+(* Deploy an implementation based on a specification *)
+Module BuildApp (Y': Impl) : App.
+  Module Y := Y'.
+  Open Local Scope hprop_scope.
+
+  Definition Q := Command.
+  Definition T  : Type := (Config * Y.T)%type.
+  Definition RR : Set  := Status.
+  Definition M := sigT (fun cfg : Config => Y.Impl.M cfg).
+  Definition rep (t: T) (m: M) : hprop :=
+    [fst t = projT1 m] * Y.rep (snd t) (projT2 m).
+
+  Definition I (m: M) : Prop := Y.Cert.T.I (Y.Cert.h (projT2 m)).
+ 
+  Definition func (q: Q) (m: M) : (RR * M) := 
+    match Y.Impl.mutate (projT2 m) q with
+      | (r, m') => (r, (@existT Config (fun cfg : Config => Y.Impl.M cfg)) (projT1 m) m')
+    end.
+
+  Definition AppIO (_ : Q) (_ : M) (_ : RR) (_ : M) : Trace := nil.
+
+  Theorem cast : forall (T U : Type) (t : T) (pf: T = U), U.
+    intros.  subst. auto.
+  Qed.
+
+  Open Local Scope stsepi_scope.
+
+  Definition inhabit_unpack' T U (inh : [T]) (f: forall t:T, [t]%inhabited = inh -> U) : [U].
+    intros. refine (
+    match inh as inh' return inh' = inh -> _ with
+      | inhabits v => fun pf => inhabits (f v pf)
+    end (refl_equal _)).
+  Qed.
+  Theorem pfCast : forall (t : T)  (m : [M])  (pf : [fst t]%inhabited = (m ~~~ projT1 m))  (m0 : M),
+    [m0]%inhabited = m -> Y.Impl.M (projT1 m0) = Y.Impl.M (fst t).
+  Proof.
+    intros. rewrite <- H in *. simpl in *. rewrite <- (pack_injective pf). auto.
+  Qed.
+
+  Definition build : forall (t : T) (m : [M]), 
+    STsep (m ~~ [fst t = projT1 m])
+          (fun res : [Y.Impl.M (fst t)] => m ~~ [fst t = projT1 m]).
+    intros. refine (pf <- shift ([fst t]%inhabited = (m ~~~ projT1 m)) <@> _ ; 
+                    {{ Return (@inhabit_unpack' _ _ m 
+                                 (fun m pf' => @cast _ _ (projT2 m) _)) }}).
+    unfold rep. rsep fail auto. rewrite H0. rsep fail auto.
+    rsep fail auto.
+    rsep fail auto.
+    instantiate (1 := (@pfCast t m pf m0 pf')). rsep fail auto.
+    sep fail auto.
+  Qed.
+
+  Definition exec (t : T) (q : Q) (m : [M]) (tr : [Trace]) :
+    STsep (tr ~~ m ~~ rep t m * traced tr * [I m]) 
+          (fun r : RR => tr ~~ m ~~ 
+            let m' := snd (func q m)
+            in  [r = fst (func q m)] * rep t m' * [I m'] * 
+            traced (AppIO q m r m' ++ tr)).
+    intros.
+    refine (pf <- shift ([fst t]%inhabited = (m ~~~ projT1 m)) <@> _ ;
+            {{ @Y.imp_mutate (fst t) (snd t) q
+                  (@inhabit_unpack' _ _ m (fun m0 pf' => @cast _ _ (projT2 m0) (@pfCast t m pf m0 pf'))) <@> _ }}).
+    unfold rep; rsep fail auto. rewrite H1. rsep fail auto.
+    rsep fail auto.
+    unfold I. unfold Y.Impl.M. unfold Y.Impl.I.    
+    pose (pack_type_inv m). instantiate (1 := tr ~~ traced tr).
+    sep fail auto.
+(* NEW
+    pose (@inhabit_unpack M (Y.Cert.T.M (fst t)) m (fun m => @Y.Cert.h (projT1 m) (projT2 m))).
+    pose (@Y.imp_mutate (fst t) (snd t) q (m ~~~ @Y.Cert.h (projT1 m) (projT2 m))).
+*)
+(* OLD
+    intros; refine ({{ Y.imp_mutate (fst t) (snd t) q (m ~~~ snd m) <@> (tr ~~ m ~~ [fst t = fst m] * traced tr * [I m]) }}).
+    unfold rep. unfold I. rsep fail auto. rewrite H1. rsep fail auto.
+    unfold rep. unfold I. rsep fail auto. subst.
+    assert (snd x0 = x1). sep fail auto. subst. rsep fail auto. rewrite H3 in *. unfold func. 
+    remember (Y.M.mutate (fst x0) (snd x0) q) as pf.
+    destruct pf. simpl in *. rsep fail auto. pose (pf2 := Y.M.PreservesI H2 q). rewrite <- Heqpf in pf2. simpl in pf2.
+    rsep fail auto.
+*)
+  Admitted.
+ 
+  Definition init :
+    STsep (__)
+          (fun tm : T * [M] => hprop_unpack (snd tm) (fun m => rep (fst tm) m * [I m])).
+    refine (res <- Y.init ;
+            {{ Return ((projT1 (snd res), (fst res)), _) }}).
+    rsep fail auto. rsep fail auto. rsep fail auto.  unfold M.
+  Admitted.
+
+  Definition cleanup : forall (t : T) (m : [M]),
+    STsep (m ~~ rep t m * [I m])
+          (fun _:unit => __).
+  Admitted.
+
+  Definition func_preserves_I : forall q m, I m -> I (snd (func q m)).
+  Admitted.
+
+End BuildApp. 
+
+
+
+(* *************************************************************************** *)
+(* Specification *)
+
+Module Spec <: Model.
+  Definition M (_:Config) : Type := list (ID * list Grade).
+  Definition I (cfg : Config) (m : M cfg) : Prop :=
+    store_inv m cfg = true.
+
+  Definition mutate (cfg: Config) (m : M cfg) (q: Command) : (Status * M cfg) :=
+    if private cfg q
+    then match q with
+           | SetGrade id pass x a g => 
+             if inbounds g a (totals cfg) 
+             then match lookup x m with
+                    | None => (ERR_NOINV, m)
+                    | Some g' => (OK, insert x (nth_set g a g') m)  
+                  end
+             else (ERR_BADGRADE, m)
+           | GetGrade id pass x a =>
+             match lookup x m with
+               | None => (ERR_NOINV, m) 
+               | Some g' => match nth_get a g' with
+                              | None => (ERR_BADGRADE, m)
+                              | Some g'' => (RET g'', m)
+                            end
+             end
+           | Average  id pass a => 
+             if validAssignment cfg a then  
+               match proj a m with
+                 | None => (ERR_NOINV, m)
+                 | Some x => (RET (avg x), m)
+               end
+               else (ERR_BADGRADE, m)
+         end
+      else (ERR_NOTPRIVATE, m).
+
+  Theorem PreservesI : forall (cfg: Config) (m : M cfg) (pfI: I m) (q: Command),
+    I (snd (mutate m q)).
+  Proof.
+    unfold I. intros. unfold mutate.
+    destruct q;
+      [ exhaustive assumption
+      | simpl in *; exhaustive assumption
+      | simpl in *; exhaustive assumption ].
+    unfold store_inv in *. symmetry in HeqRM. all.
+    Hint Resolve insert_preserves_noduples.
+    Hint Resolve insert_preserves_total_dec.
+    Hint Resolve insert_preserves_inv.
+    each; auto.
+  Qed.
+
+End Spec.
+
+(** Spec is isomorphic to itself **)
+Module SpecHomomorphism : ModelHomomorphism with Module S := Spec with Module T := Spec.
+
+  Module S := Spec.
+  Module T := Spec.
+
+  Definition h (cfg: Config) (m: S.M cfg) : T.M cfg := m.
+   
+  Theorem InvPres : forall cfg (m: S.M cfg), S.I m -> T.I (h m).
+  Proof.
+    unfold h; auto.
+  Qed.
+
+  Theorem ObserveEq : forall cfg (m: S.M cfg), S.I m ->
+    forall q, fst (S.mutate m q) = fst (T.mutate (h m) q).
+  Proof.
+    unfold h; auto.
+  Qed.
+
+  Theorem StatePres : forall cfg (m: S.M cfg), S.I m ->
+    forall q, h (snd (S.mutate m q)) = snd (T.mutate  (h m) q).
+  Proof.
+    unfold h; auto.
+  Qed.
+
+End SpecHomomorphism.
+
+
+(* **************************************************************************************** *)
+(* Store Implementation *)
+(**
+Module StoreImplModel <: Model.
+  Import StoreModel.
+  Import GradesStoreMapping.
+
+  Definition M (cfg : Config) : Type := Table (S (length (totals cfg))).
+  Definition I (cfg : Config) (m : M cfg) : Prop :=
+    store_inv (Table2List m) cfg = true.
+
+  Definition mutate (cfg: Config) (m : M cfg) (q: Command) : (Status * M cfg) :=
+    if private cfg q
+    then match q with
+           | SetGrade id pass x a g =>
+             if inbounds g a (totals cfg)
+               then (OK, update (set_query x a g) m)
+               else (ERR_BADGRADE, m)
+           | GetGrade id pass x a =>
+             (match nthget a (select (get_query x cfg) m) with 
+                | None => ERR_NOINV
+                | Some None => ERR_BADGRADE
+                | Some (Some g') => RET g'
+              end, m)
+           | Average  id pass assign =>
+             (match validAssignment cfg assign with
+                | right _ => ERR_BADGRADE
+                | left pfx2 =>
+                  let projs := project (GET_COL (Lt.lt_n_S _ _ pfx2)) m in
+                  let agg := aggregate (fun (a : nat) (x0 : Tuple 1) => fst x0 + a) 0 projs in
+                  RET (divcheck0 agg (length (students cfg)))
+              end, m)
+         end
+      else (ERR_NOTPRIVATE, m).
+
+  Lemma InvDenote : forall cfg m,
+    store_inv1 m cfg = true
+    -> forall x, In x m -> length (snd x) = length (totals cfg).
+    induction m.
+      simpl. intros. inversion H0.
+      intros. simpl in *; all; destruct H0.
+        subst; apply bounded_length; auto.
+        apply IHm; auto.
+  Qed.
+
+  Lemma Table2List_List2Table : forall m l,
+    (forall x, In x m -> length (snd x) = l) ->
+    Table2List (List2Table m l) = m.
+    induction m.
+      auto.
+      intros. assert (length (snd a) = l). apply H; apply in_eq.
+      simpl. destruct a. inv auto. simpl. inv auto. clear H. generalize dependent l0. clear.
+      induction l.
+        simpl. destruct l0; simpl in *; auto; congruence.
+        simpl. destruct l0. simpl. intros. congruence. simpl. intros. inv auto.
+  Qed.
+
+  Lemma dec : forall (a b : ID * list Grade), {a = b} + {a <> b}.
+    do 3 decide equality.
+  Qed.
+
+  Theorem PreservesI : forall (cfg: Config) (m : M cfg) (pfI: I m) (q: Command),
+    I (snd (mutate m q)).
+  Proof.
+    intros. unfold mutate. unfold I in *. destruct q; exhaustive auto. 
+    pose (@SetGrade_OK_store (cfg, Table2List m) i p i0 a g). simpl in e. rewrite List2Table_Table2List in e. rewrite e; try solve [ subst; auto ]. clear e.
+    rewrite <- HeqRM. rewrite <- HeqRM0. destruct (@private_lookup i0 (Table2List m) cfg i p a g); auto. subst. auto.
+    rewrite H. simpl. rewrite Table2List_List2Table.
+    unfold store_inv in *. all.
+    Hint Resolve insert_preserves_total_dec.
+    Hint Resolve insert_preserves_noduples.
+    Hint Resolve insert_preserves_inv.
+    each; auto.
+    assert (length (nth_set g a x) = length (totals cfg)).
+    cut (length x = length (totals cfg)).
+    clear. destruct cfg. simpl. clear. generalize dependent totals0. generalize dependent a. 
+    induction x.
+      auto.
+      simpl; intros. destruct totals0; try (simpl in *; congruence). simpl in *. 
+        destruct a0. auto. simpl. rewrite (IHx a0 totals0); auto.
+    unfold store_inv in pfI. all. generalize F1 H. clear. generalize m. generalize cfg. clear.
+    induction m.
+      simpl. congruence.
+      destruct a. simpl. intros. all. destruct (id_dec i0 n).
+        inversion H. rewrite H1 in *. apply bounded_length; auto.
+        apply IHm; auto.
+    unfold store_inv in *. all. generalize (InvDenote _ _ F1). 
+    generalize H. generalize H0. generalize x. generalize m. generalize cfg. clear.
+    induction m.
+      simpl. congruence.
+      simpl. destruct a0. simpl. intros. destruct (id_dec n i0); destruct (id_dec i0 n); try congruence.
+        inversion H. rewrite H4 in *. 
+        apply (decideable_in _ dec) in H2. destruct H2. rewrite <- H2. simpl; auto. eapply H1; eauto. right; tauto.
+        destruct H2. apply H1. left; auto.
+        eapply IHm; eauto. 
+  Qed.
+      
+End StoreImplModel.
+
+(** A morphism between models **)
+Module StoreHomomorphism : ModelHomomorphism with Module S := Spec
+                                             with Module T := StoreImplModel.
+  Module S := Spec.
+  Module T := StoreImplModel.
+  Import StoreModel.
+  Import GradesStoreMapping.
+
+  Definition h (cfg : Config) (sm : S.M cfg) : T.M cfg :=
+    List2Table sm (length (totals cfg)).
+   
+
+  Lemma decideable_in : forall T (dec : forall a b : T, {a = b} + {a <> b}) (a x : T) b,
+    In x (a :: b) -> a = x \/ (x <> a /\ In x b).
+    intros. destruct (dec x a); auto. 
+    right. destruct H. congruence. auto.
+  Qed.
+
+  Lemma dec : forall (a b : ID * list Grade), {a = b} + {a <> b}.
+    do 3 decide equality.
+  Qed.
+
+  Theorem InvPres : forall cfg (m: S.M cfg), S.I m -> T.I (h m).
+  Proof.
+    intros; unfold T.I, S.I,h in *. rewrite T.Table2List_List2Table; auto.
+    intros. unfold store_inv in H. all. clear F F0 H. destruct x. induction m.
+      simpl in *. firstorder.
+      apply (decideable_in dec) in H0.
+      simpl in *. destruct H0. subst. all. simpl in *. apply bounded_length; auto. 
+        destruct H. apply IHm; auto. all. auto.
+  Qed.
+
+  (* h (S.mutate x) = T.mutate (h x) *)
+  Opaque GET_COL.
+  Theorem ObserveEq : forall cfg (m: S.M cfg), S.I m ->
+    forall q,  fst (S.mutate m q) = fst (T.mutate  (h m) q).
+  Proof.
+    intros. unfold S.I in *. unfold S.mutate, T.mutate. simpl projT1. simpl projT2.
+    remember (private cfg q) as PVT; destruct PVT; auto.
+    destruct q.
+      (** SET **)
+      destruct (inbounds g a (totals cfg)); auto. simpl. destruct (private_lookup i0 m cfg i p a g); auto. rewrite H0. auto.
+      (** GET **)
+      unfold h.
+      destruct (private_lookup i0 m cfg i p a 0); auto. rewrite H0.
+      pose (grade_count _ _ H _ H0). symmetry in e. destruct (lookup_select m cfg i0 H0). rewrite H1. simpl.
+      remember (nthget' _ a (List2Tuple' x (length (totals cfg)))) as NTH. destruct NTH. symmetry in HeqNTH.
+      rewrite (@gg_ret _ _ _ _ e HeqNTH). auto. 
+      symmetry in HeqNTH. rewrite (gg_bad _ _ e HeqNTH). auto.
+      (** AVG **)
+      unfold h. simpl. destruct (validAssignment cfg a); auto.
+      pose (@AvgRet (RET
+        (divcheck0
+          (aggregate (fun (a0 : nat) (x0 : Tuple 1) => fst x0 + a0) 0
+            (project (GET_COL (Lt.lt_n_S a (length (totals cfg)) l))
+              (List2Table m (length (totals cfg))))) 
+          (length (students cfg)))) (project (GET_COL (Lt.lt_n_S a (length (totals cfg)) l))
+            (List2Table m (length (totals cfg)))) (aggregate (fun (a0 : nat) (x0 : Tuple 1) => fst x0 + a0) 0
+              (project (GET_COL (Lt.lt_n_S a (length (totals cfg)) l))
+                (List2Table m (length (totals cfg))))) m cfg a i p l). unfold Tuple in e. rewrite e; auto. clear e. 
+      simpl. simpl in HeqPVT. rewrite <- HeqPVT. destruct (validAssignment cfg a). destruct (proj a m); auto. elimtype False. omega.
+  Qed.
+
+  Theorem StatePres : forall cfg (m: S.M cfg), S.I m ->
+    forall q, h (snd (S.mutate m q)) = snd (T.mutate (h m) q).
+  Proof.
+    unfold S.I, S.mutate, T.mutate, h. simpl projT1; simpl projT2.
+    intros; remember (private cfg q) as PVT; destruct PVT; auto.
+    destruct q;
+      [ | exhaustive auto | exhaustive auto ].
+      remember (inbounds g a (totals cfg)) as IB; destruct IB; auto.
+      pose (@SetGrade_OK_store (cfg,m) i p i0 a g). simpl in e. rewrite e; auto. clear e.
+      destruct (private_lookup i0 m cfg i p a 0); auto. rewrite H0. simpl.
+      unfold h. simpl in HeqPVT. rewrite <- HeqPVT. auto. rewrite <- HeqIB. auto.
+  Qed.
+
+End StoreHomomorphism.
+
+Module GbStoreImpl  (s: Store)  <: Impl. (* had name clash *)
+  Module M := StoreImplModel.
+  Export M.
+  Definition T := s.t.
+  Open Scope hprop_scope.
+
+  Definition rep (cfg : Config) (t: T) (m: M.M cfg) : hprop :=
+    s.rep t m.
+
+  Open Local Scope hprop_scope.
+
+  Definition imp_mutate : forall cfg (t: T ) q (m: [M.M cfg]),
+    STsep (m ~~ rep t m * [M.I m] ) 
+          (fun r : Status => m ~~ let (r', m') := (M.mutate m q)
+                                  in  [r' = r] * rep t m').
+    intros.
+  Admitted.
+
+End GbStoreImpl.
+
+
+(* ************************************************************************************************ *)
+(* Certification *)
+
+Module CertifiedImpl (s: Store) : Impl.
+ Module M := Spec.
+ Module TheImpl := GbStoreImpl s.
+ Definition T := TheImpl.T.
+ Definition rep (cfg : Config) (t: TheImpl.T) (m: Spec.M cfg) : hprop :=
+   @TheImpl.rep cfg t (StoreHomomorphism.h m).
+
+ Open Scope hprop_scope.
+ Definition imp_mutate : forall cfg (t: T) q (m: [M.M cfg]),
+    STsep (m ~~ @rep cfg t m * [M.I m] ) 
+          (fun r : Status => m ~~ let (r', m') := (M.mutate m q)
+                                  in  [r' = r] * @rep cfg t m').
+    refine (fun cfg t q m =>
+      {{ TheImpl.imp_mutate t q (m ~~~ @StoreHomomorphism.h cfg m) }}).
+    
+    unfold rep, TheImpl.rep,M.I. rsep fail auto. pose (@StoreHomomorphism.InvPres cfg x H0). rsep fail auto.
+    unfold rep. rsep fail auto. (** TODO: Generalization required here **)
+ Admitted.
+
+End CertifiedImpl.
+
+
+Module someStore : Store := ListStore.
+Module theImpl : Impl := GbStoreImpl someStore.
+Module theApp : App := BuildApp theImpl.
+
+(*
+Module StoreImpl <: Impl with Module M := TupleModel.
+  Module M := TupleModel.
+End StoreImpl.
+
+
+(* these wrappers may come in handy 
+   for above. *)
+Module WrapModel (X: Model).
+  Export X.
+
+  Definition wrap cfg q m (pf_I: I cfg m) :=
+    match P_dec cfg q with
+      | left  pf_P => match E_dec cfg q with
+                        | left  pf_E => mutate cfg q m  
+                        | right pf_badgrade => (ERR_BADGRADE, m) 
+                      end
+      | right pf_notpriv => (ERR_NOTPRIVATE, m)
+    end.
+End WrapModel.
+
+Require Import Ynot.
+Module WrapImpl (X: Model) (Y: Impl).
+ Module Z := Y X.
+ Export Z.
+ Module W := WrapModel X.
+ Export W.
+
+ Open Local Scope stsepi_scope.
+ Open Local Scope hprop_scope.
+ Definition imp_wrap cfg t q m : 
+  STsep (m ~~ rep t m * [I cfg m] * [P cfg q] * [E cfg q]) 
+   (fun r : Status => m ~~ Exists pf1 :@ I cfg m, 
+                           let (r', m') := (wrap q pf1 )
+                           in  [r' = r] * rep t m').
+ Admitted. 
+End WrapImpl.
+
+Require Import Ynot.
+ 
+
+
+Require Import Store.
+
+(* And we need to do this as well
+Module StoreImpl (s: Store) : Impl TupleModel .
+ 
+End StoreImpl.
+*)
+**)
+
+(**
+Module Test (H: ModelHomomorphism). (* sanity check *)
+ Export H.
+  Theorem thm1 : forall cfg (m: S.M cfg) q, S.I m -> T.I (snd (T.mutate (h m) q)).
+   intros. apply T.PreservesI. pose (hCorrect H). destruct a. assumption.
+ Qed.
+End Test.
+**)
+
+**)
