examples/servers/UdpClient.v
@@ -1,0 +1,101 @@
+Require Import List Ascii.
+Require Import Ynot.
+Require Import IO Net FS.
+
+Open Local Scope hprop_scope.
+Open Local Scope stsepi_scope.
+Open Local Scope char_scope.
+
+Set Implicit Arguments.
+
+Inductive trace (local remote : Net.SockAddr) : IO.Trace -> Prop :=
+| NilCorrect : trace local remote nil
+| ConsCorrect : forall data reply past wait, trace local remote past -> 
+  (forall msg, ~In (UDP.Recd local remote msg) wait) ->
+  trace local remote 
+      (WroteString stdout reply ++
+       UDP.Recd local remote reply :: wait ++ UDP.Sent local remote data :: 
+       ReadLine stdin data ++ past).
+
+Lemma proj_inv : forall (T1 T2 : Type) (a b : T1) (c d : T2),
+  (a,c) = (b,d) -> a = b /\ c = d.
+  intros; inversion H; auto.
+Qed.
+
+Definition waitReceive : forall (local remote : Net.SockAddr) (tr : [Trace]),
+  STsep (tr ~~ IO.traced tr)
+        (fun res:(list ascii * [Trace]) => tr ~~ 
+          im :~~ (snd res) in IO.traced (UDP.Recd local remote (fst res) :: (im ++ tr))).
+  intros. refine (
+    {{Fix (fun im => im ~~ tr ~~ IO.traced (im ++ tr))
+        (fun _ (res:list ascii * [Trace]) => tr ~~
+           im :~~ (snd res) in IO.traced (UDP.Recd local remote (fst res) :: (im ++ tr)))
+        (fun self im => 
+           reply <- UDP.recv local (inhabit_unpack2 im tr (fun im tr => im ++ tr)); 
+           if sock_eq remote (fst reply) then 
+             {{Return (snd reply, im)}}
+           else
+             {{self (im ~~~ (UDP.Recd local (fst reply) (snd reply)) :: im)}}
+         ) [@nil Action]%inhabited}});
+  solve [ sep fail auto
+        | sep fail auto; apply proj_inv in H; destruct H; sep fail auto ].
+Qed.
+
+Definition iter : forall (local remote : Net.SockAddr) (tr : [Trace]),
+  STsep (tr ~~ IO.traced tr)
+        (fun _:unit => tr ~~ Exists request :@ list ascii, Exists reply :@ list ascii, Exists q :@ Trace,
+          IO.traced (WroteString FS.stdout reply  ++
+            (UDP.Recd local remote reply :: (q ++ UDP.Sent local remote request ::
+              (ReadLine FS.stdin request ++ tr))))).
+  intros. refine (
+    ln <- readline FS.stdin FS.ro_readable tr;
+    UDP.send local remote ln (tr ~~~ ReadLine FS.stdin ln ++ tr);;
+    reply <- waitReceive local remote (tr ~~~ UDP.Sent local remote ln :: (ReadLine FS.stdin ln ++ tr)) <@> _;
+    writeline FS.stdout (fst reply) FS.wo_writeable (inhabit_unpack2 tr (snd reply) 
+      (fun tr q => (UDP.Recd local remote (fst reply)) :: q ++ (UDP.Sent local remote ln ::
+        (ReadLine FS.stdin ln ++ tr))));;
+    {{Return tt}}).
+  sep fail auto.
+  sep fail auto.
+  sep fail auto.
+  sep fail auto.
+  sep fail auto.
+  sep fail auto.
+  sep fail auto. destruct reply. simpl in *. pose (pack_type_inv i). destruct e. rewrite -> H in H1. sep fail auto.
+  sep fail auto.
+  sep fail auto.
+  intros; inhabiter. simpl in *. destruct reply; simpl in *. pose (pack_type_inv i). destruct e. rewrite H in H0. rewrite H1 in H0. simpl in *. apply pack_injective in H0. rewrite <- H0. sep fail auto.
+Qed.
+
+Theorem list_no_cycle : forall (T : Type) (l1 l2 : list T),
+  l2 <> nil -> l1 <> l2 ++ l1.
+  induction l1. 
+    auto.
+    intros. rewrite <- app_nil_end. auto.
+    intros. destruct l2. congruence. unfold not in *. intros. inversion H0.
+    rewrite <- nil_cons_app in H3. eapply IHl1. instantiate (1 := (l2 ++ t :: nil)). intros. destruct l2; discriminate.
+     auto.
+Qed.
+
+Theorem list_no_cycle' : forall (T : Type) (l1 l2 : list T),
+  l2 <> nil -> l2 ++ l1 <> l1.
+  intros; pose (@list_no_cycle T l1 l2); unfold not in *; auto.
+Qed.
+
+Definition client : forall (local remote : Net.SockAddr) (tr : [Trace]),
+  STsep (tr ~~ [trace local remote tr] * IO.traced tr)
+        (fun _:unit => tr ~~ Exists v :@ Trace, [v <> tr] * [trace local remote tr] *
+             IO.traced v).
+  intros. refine ({{iter local remote tr <@> (tr ~~ [trace local remote tr])}}).
+  sep fail auto.
+  intros; inhabiter. sep fail auto. assert (WroteString stdout v1 ++
+      (UDP.Recd local remote v1
+       :: v2 ++ UDP.Sent local remote v0 :: ReadLine stdin v0 ++ x) <> x).
+  unfold WroteString, ReadLine. assert ((WroteString stdout v1 ++
+   UDP.Recd local remote v1
+   :: v2 ++
+      UDP.Sent local remote v0
+      :: ReadLine stdin v0) ++ x <> x).
+  eapply list_no_cycle'. firstorder. rewrite app_ass in H3. simpl in *. rewrite app_ass in H3. simpl in *. firstorder.
+  sep fail auto.
+Qed.
